src/definitions3.lean
@@ -1,0 +1,91 @@
+-- definitions that are used by the lemmas but not referenced by the soundness theorem
+
+import .definitions2
+
+-- top-level calls and quantifiers in positive and negative positions
+mutual inductive prop.has_call_p, prop.has_call_n
+
+with prop.has_call_p: calltrigger → prop → Prop
+| calltrigger {x: term}                                 : prop.has_call_p ⟨x⟩ (prop.call x)
+| not {P: prop} {c: calltrigger}                        : prop.has_call_n c P  → prop.has_call_p c P.not
+| and₁ {P₁ P₂: prop} {c: calltrigger}                   : prop.has_call_p c P₁ → prop.has_call_p c (P₁ ⋀ P₂)
+| and₂ {P₁ P₂: prop} {c: calltrigger}                   : prop.has_call_p c P₂ → prop.has_call_p c (P₁ ⋀ P₂)
+| or₁ {P₁ P₂: prop} {c: calltrigger}                    : prop.has_call_p c P₁ → prop.has_call_p c (P₁ ⋁ P₂)
+| or₂ {P₁ P₂: prop} {c: calltrigger}                    : prop.has_call_p c P₂ → prop.has_call_p c (P₁ ⋁ P₂)
+
+with prop.has_call_n: calltrigger → prop → Prop
+| not {P: prop} {c: calltrigger}                        : prop.has_call_p c P  → prop.has_call_n c P.not
+| and₁ {P₁ P₂: prop} {c: calltrigger}                   : prop.has_call_n c P₁ → prop.has_call_n c (P₁ ⋀ P₂)
+| and₂ {P₁ P₂: prop} {c: calltrigger}                   : prop.has_call_n c P₂ → prop.has_call_n c (P₁ ⋀ P₂)
+| or₁ {P₁ P₂: prop} {c: calltrigger}                    : prop.has_call_n c P₁ → prop.has_call_n c (P₁ ⋁ P₂)
+| or₂ {P₁ P₂: prop} {c: calltrigger}                    : prop.has_call_n c P₂ → prop.has_call_n c (P₁ ⋁ P₂)
+
+-- sets of calls
+def calls_p (P: prop): set calltrigger := λc, prop.has_call_p c P
+def calls_n (P: prop): set calltrigger := λc, prop.has_call_n c P
+
+mutual inductive prop.has_quantifier_p, prop.has_quantifier_n
+
+with prop.has_quantifier_p: callquantifier → prop → Prop
+| callquantifier {x: var} {P: prop}           : prop.has_quantifier_p ⟨x, P⟩ (prop.forallc x P)
+| not {P: prop} {q: callquantifier}           : prop.has_quantifier_n q P  → prop.has_quantifier_p q P.not
+| and₁ {P₁ P₂: prop} {q: callquantifier}      : prop.has_quantifier_p q P₁ → prop.has_quantifier_p q (P₁ ⋀ P₂)
+| and₂ {P₁ P₂: prop} {q: callquantifier}      : prop.has_quantifier_p q P₂ → prop.has_quantifier_p q (P₁ ⋀ P₂)
+| or₁ {P₁ P₂: prop} {q: callquantifier}       : prop.has_quantifier_p q P₁ → prop.has_quantifier_p q (P₁ ⋁ P₂)
+| or₂ {P₁ P₂: prop} {q: callquantifier}       : prop.has_quantifier_p q P₂ → prop.has_quantifier_p q (P₁ ⋁ P₂)
+
+with prop.has_quantifier_n: callquantifier → prop → Prop
+| not {P: prop} {q: callquantifier}           : prop.has_quantifier_p q P  → prop.has_quantifier_n q P.not
+| and₁ {P₁ P₂: prop} {q: callquantifier}      : prop.has_quantifier_n q P₁ → prop.has_quantifier_n q (P₁ ⋀ P₂)
+| and₂ {P₁ P₂: prop} {q: callquantifier}      : prop.has_quantifier_n q P₂ → prop.has_quantifier_n q (P₁ ⋀ P₂)
+| or₁ {P₁ P₂: prop} {q: callquantifier}       : prop.has_quantifier_n q P₁ → prop.has_quantifier_n q (P₁ ⋁ P₂)
+| or₂ {P₁ P₂: prop} {q: callquantifier}       : prop.has_quantifier_n q P₂ → prop.has_quantifier_n q (P₁ ⋁ P₂)
+-- universal quantifiers below existential quantifiers only occur in positive positions,
+-- so can be skolemized instead of instantiated
+
+-- sets of quantifiers
+def quantifiers_p (P: prop): set callquantifier := λc, has_quantifier_p c P
+def quantifiers_n (P: prop): set callquantifier := λc, has_quantifier_n c P
+
+ -- propositions without call triggers or quantifiers do not participate in instantiations
+def no_instantiations(P: prop): Prop := (calls_p P = ∅) ∧ (calls_n P = ∅) ∧
+                                        (quantifiers_p P = ∅) ∧ (quantifiers_n P = ∅)
+
+-- set of calltriggers after substitution
+def calltrigger.subst (σ: env) (c: calltrigger): calltrigger := ⟨term.subst_env σ c.x⟩
+def calls_p_subst (σ: env) (P: prop): set calltrigger := (calltrigger.subst σ) '' calls_p P
+def calls_n_subst (σ: env) (P: prop): set calltrigger := (calltrigger.subst σ) '' calls_n P
+
+-- runtime verification of stacks
+
+inductive stack.vcgen : stack → propctx → Prop
+notation `⊢ₛ` s `:` Q : 10 := stack.vcgen s Q
+
+| top {R: spec} {P: prop} {σ: env} {e: exp} {Q: propctx}:
+    (⊢ σ : P) →
+    FV R.to_prop ⊆ FV P →
+    (σ ⊨ R.to_prop.instantiated_n.erased_n) →
+    (R ⋀ P ⊢ e : Q) →
+    (⊢ₛ (R, σ, e) : P ⋀ Q)
+
+| cons {P₁ P₂ P₃: prop} {s: stack} {σ₁ σ₂: env}
+       {f fx g x y: var} {R₁ R₂ S₂: spec} {e₁ e₂: exp} {v: value} {Q₁ Q₂ Q₂': propctx}:
+    (⊢ₛ s : Q₂') →
+    y ∉ σ₁ →
+    (⊢ σ₁ : P₁) →
+    (⊢ σ₂ : P₂ ) →
+    (⊢ (σ₂[f↦value.func f fx R₂ S₂ e₂ σ₂][fx↦v]) : P₃) →
+    FV R₁.to_prop ⊆ FV P₁ →
+    (σ₁ ⊨ R₁.to_prop.instantiated_n.erased_n) →
+    (σ₁ g = value.func f fx R₂ S₂ e₂ σ₂) →
+    (σ₁ x = v) →
+    (R₁ ⋀ P₁ ⋀ prop.call g x ⋀ prop.post g x ⋀ y ≡ term.app g x ⊢ e₁ : Q₁) →
+    (P₂ ⋀ spec.func f fx R₂ S₂ ⋀ R₂ ⊢ e₂ : Q₂) →
+    (∀σ' t, (σ' ⊨ (Q₂' t).instantiated_n.erased_n) → σ' ⊨ (P₃ ⋀ (Q₂ t)).instantiated_n.erased_n) →
+    (∀v: value, FV (P₃ ⋀ (Q₂ v)) ⊆ FV (Q₂' v)) →
+    ⟪ prop.implies (R₁ ⋀ P₁ ⋀ prop.call g x) (term.unop unop.isFunc g ⋀ prop.pre g x) ⟫ →
+    ((R₂, σ₂[f↦value.func f fx R₂ S₂ e₂ σ₂][fx↦v], e₂) ⟶* s) →
+    (⊢ₛ (s · [R₁, σ₁, letapp y = g[x] in e₁]) : P₁ ⋀
+          propctx.exis y (prop.call g x ⋀ prop.post g x ⋀ y ≡ term.app g x ⋀ Q₁))
+
+notation `⊢ₛ` s `:` Q : 10 := stack.vcgen s Q
