src/substitution.lean
@@ -1,6 +1,6 @@
 -- lemmas about substitution
 
-import .definitions1 .freevars
+import .definitions1 .freevars .others
 
 lemma env.contains.inv {σ: env} {x y: var} {v: value}: x ∈ (σ[y↦v]) → (x = y ∨ x ∈ σ) :=
   assume x_in: x ∈ (σ[y↦v]),
@@ -190,6 +190,13 @@ instance {σ: env} {x: var} : decidable (env.contains σ x) :=
     have x ∈ σ, from env.contains_apply_equiv.right.mp this,
     is_true this
   ) rfl
+
+lemma term.subst.congr {x: var} {v: value} {t₁ t₂: term}: (t₁ = t₂) → (term.subst x v t₁ = term.subst x v t₂) :=
+  begin
+    assume h1,
+    congr,
+    from h1
+  end
 
 lemma env.contains_without.inv {σ: env} {x y: var}:
       (x ∈ σ.without y) → (x ≠ y) ∧ x ∈ σ :=
@@ -399,6 +406,37 @@ lemma env.without_equiv {σ: env} {x y: var} {v: value}:
     from h18
   end
 
+lemma env.not_in_without {σ: env} {x y: var}: x ∉ σ → x ∉ σ.without y :=
+  begin
+    assume h1,
+
+    induction σ with σ' z v' ih,
+
+    unfold env.without,
+    assume h4,
+    cases h4,
+
+    unfold env.without,
+    by_cases (z = y) with h4,
+    simp[h4],
+    assume h5,
+    have h6, from env.contains_without.inv h5,
+    have : x ∈ (σ'[z↦v']), from env.contains.rest h6.right,
+    contradiction,
+
+    simp[h4],
+    assume h5,
+    have h6, from env.contains.inv h5,
+    cases h6 with h7 h8,
+    rw[h7] at h1,
+    have : z ∈ (σ'[z↦v']), from env.contains.same,
+    contradiction,
+
+    have h9, from env.contains_without.inv h8,
+    have : x ∈ (σ'[z↦v']), from env.contains.rest h9.right,
+    contradiction
+  end
+
 lemma env.not_contains_without {σ: env} {x: var}: x ∉ σ.without x :=
   assume : x ∈ σ.without x,
   have (x ≠ x) ∧ x ∈ σ, from env.contains_without.inv this,
@@ -492,6 +530,21 @@ lemma unchanged_of_subst_nonfree_term {t: term} {x: var} {v: value}:
     )
   end
 
+lemma unchanged_of_subst_env_nonfree_term {t: term}:
+    closed t → (∀σ, term.subst_env σ t = t) :=
+  assume x_not_free: (∀x, x ∉ FV t),
+  assume σ: env,
+  begin
+    induction σ with σ' x v ih,
+
+    show (term.subst_env env.empty t = t), by unfold term.subst_env,
+
+    show (term.subst_env (σ'[x↦v]) t = t), by calc
+        term.subst_env (σ'[x↦v]) t = term.subst x v (term.subst_env σ' t) : by unfold term.subst_env
+                               ... = term.subst x v t : by rw[ih]
+                               ... = t : unchanged_of_subst_nonfree_term (x_not_free x)
+  end
+
 lemma term.subst.var.same {x: var} {v: value}: term.subst x v x = v :=
   have h: term.subst x v (term.var x) = (if x = x then v else x), by unfold term.subst,
   have (if x = x then (term.value v) else (term.var x)) = (term.value v), by simp,
@@ -502,6 +555,12 @@ lemma term.subst.var.diff {x y: var} {v: value}: (x ≠ y) → (term.subst x v y
   have h: term.subst x v (term.var y) = (if x = y then v else y), by unfold term.subst,
   have (if x = y then (term.value v) else (term.var y)) = (term.var y), by simp[x_neq_y],
   show term.subst x v y = y, from eq.trans h this
+
+lemma term.substt.var.diff {x y: var} {t: term}: (x ≠ y) → (term.substt x t y = y) :=
+  assume x_neq_y: x ≠ y,
+  have h: term.substt x t (term.var y) = (if x = y then t else y), by unfold term.substt,
+  have (if x = y then t else (term.var y)) = (term.var y), by simp[x_neq_y],
+  show term.substt x t y = y, from eq.trans h this
 
 lemma unchanged_of_subst_nonfree_prop {P: prop} {x: var} {v: value}:
     x ∉ FV P → (prop.subst x v P = P) :=
@@ -933,6 +992,100 @@ lemma free_of_subst_term {t: term} {x y: var} {v: value}:
     )
   end
 
+lemma free_of_substt_same_term {t t': term} {x: var}:
+          free_in_term x (term.substt x t' t) → free_in_term x t' :=
+  assume x_free_in_subst: free_in_term x (term.substt x t' t),
+  begin
+    induction t with v' z unop t₁ t₁_ih binop t₂ t₃ t₂_ih t₃_ih t₄ t₅ t₄_ih t₅_ih,
+    show free_in_term x t', from (
+      have term.substt x t' (term.value v') = v', by unfold term.substt,
+      have free_in_term x v', from this ▸ x_free_in_subst,
+      show free_in_term x t', from absurd this free_in_term.value.inv
+    ),
+    show free_in_term x t', from (
+      have hite: term.substt x t' (term.var z) = (if x = z then t' else z), by unfold term.substt,
+      if x_is_z: x = z then
+        have term.substt x t' (term.var z) = t', by { simp[x_is_z] at hite, rw[x_is_z], from hite },
+        show free_in_term x t', from this ▸ x_free_in_subst
+      else
+        have term.substt x t' (term.var z) = z, by { simp[x_is_z] at hite, from hite },
+        have free_in_term x z, from this ▸ x_free_in_subst,
+        have x_iss_z: x = z, from free_in_term.var.inv this,
+        show free_in_term x t', from absurd x_iss_z x_is_z
+    ),
+    show free_in_term x t', from (
+      have term.substt x t' (term.unop unop t₁) = term.unop unop (term.substt x t' t₁), by unfold term.substt,
+      have free_in_term x (term.unop unop (term.substt x t' t₁)), from this ▸ x_free_in_subst,
+      have free_in_term x (term.substt x t' t₁), from free_in_term.unop.inv this,
+      show free_in_term x t', from t₁_ih this
+    ),
+    show free_in_term x t', from (
+      have term.substt x t' (term.binop binop t₂ t₃) = term.binop binop (term.substt x t' t₂) (term.substt x t' t₃),
+      by unfold term.substt,
+      have free_in_term x (term.binop binop (term.substt x t' t₂) (term.substt x t' t₃)), from this ▸ x_free_in_subst,
+      have free_in_term x (term.substt x t' t₂) ∨ free_in_term x (term.substt x t' t₃),
+      from free_in_term.binop.inv this,
+      or.elim this (
+        assume : free_in_term x (term.substt x t' t₂),
+        show free_in_term x t', from t₂_ih this
+      ) (
+        assume : free_in_term x (term.substt x t' t₃),
+        show free_in_term x t', from t₃_ih this
+      )
+    ),
+    show free_in_term x t', from (
+      have term.substt x t' (term.app t₄ t₅) = term.app (term.substt x t' t₄) (term.substt x t' t₅),
+      by unfold term.substt,
+      have free_in_term x (term.app (term.substt x t' t₄) (term.substt x t' t₅)), from this ▸ x_free_in_subst,
+      have free_in_term x (term.substt x t' t₄) ∨ free_in_term x (term.substt x t' t₅), from free_in_term.app.inv this,
+      or.elim this (
+        assume : free_in_term x (term.substt x t' t₄),
+        show free_in_term x t', from t₄_ih this
+      ) (
+        assume : free_in_term x (term.substt x t' t₅),
+        show free_in_term x t', from t₅_ih this
+      )
+    )
+  end
+
+lemma free_of_subst_env_term_step {t: term} {σ: env} {x y: var} {v: value}:
+        free_in_term x (term.subst_env (σ[y↦v]) t) → x ≠ y ∧ free_in_term x (term.subst_env σ t) :=
+  assume x_free: free_in_term x (term.subst_env (σ[y↦v]) t),
+  have term.subst_env (σ[y↦v]) t = term.subst y v (term.subst_env σ t), by unfold term.subst_env,
+  have free_in_term x (term.subst y v (term.subst_env σ t)), from this ▸ x_free,
+  show x ≠ y ∧ free_in_term x (term.subst_env σ t), from free_of_subst_term this
+
+lemma free_of_subst_env_term {t: term} {σ: env} {x: var}:
+        free_in_term x (term.subst_env σ t) → free_in_term x t ∧ x ∉ σ :=
+  assume x_free_in_subst: free_in_term x (term.subst_env σ t),
+  begin
+    induction σ with σ' y v ih,
+    show free_in_term x t ∧ x ∉ env.empty, from (
+      have h2: x ∉ env.empty, by begin
+        assume : x ∈ env.empty,
+        have h3: env.contains env.empty x, from this,
+        cases h3
+      end,
+      have term.subst_env env.empty t = t, by unfold term.subst_env,
+      show free_in_term x t ∧ x ∉ env.empty, from ⟨this ▸ x_free_in_subst, h2⟩
+    ),
+    show free_in_term x t ∧ x ∉ (σ'[y↦v]), from (
+      have h1: x ≠ y ∧ free_in_term x (term.subst_env σ' t),
+      from free_of_subst_env_term_step x_free_in_subst,
+      have h2: free_in_term x t ∧ x ∉ σ', from ih h1.right,
+      have h3: x ∉ (σ'[y↦v]), by begin
+        assume : x ∈ (σ'[y↦v]),
+        have h3: env.contains (σ'[y↦v]) x, from this,
+        cases h3,
+        have h4: x ≠ x, from h1.left,
+        contradiction,
+        have h5: ¬ env.contains σ' x, from h2.right,
+        contradiction
+      end,
+      show free_in_term x t ∧ x ∉ (σ'[y↦v]), from ⟨h2.left, h3⟩
+    )
+  end
+
 lemma free_of_subst_prop {P: prop} {x y: var} {v: value}:
           free_in_prop x (prop.subst y v P) → x ≠ y ∧ free_in_prop x P :=
   assume x_free_in_subst: free_in_prop x (prop.subst y v P),
@@ -1319,6 +1472,21 @@ begin
   )
 end
 
+lemma term.subst_env.closed {σ: env} {t: term}: closed t → (term.subst_env σ t = t) :=
+begin
+  assume t_closed: closed t,
+  induction σ with σ' x v' ih,
+  show (term.subst_env env.empty t = t), by unfold term.subst_env,
+  show (term.subst_env (σ'[x↦v']) t = t), from (
+    have h: term.subst_env σ' t = t, from ih,
+    have term.subst_env (σ'[x↦v']) t = term.subst x v' (term.subst_env σ' t), by unfold term.subst_env,
+    have h2: term.subst_env (σ'[x↦v']) t = term.subst x v' t,
+    from @eq.subst term (λa, term.subst_env (σ'[x↦v']) t = term.subst x v' a) (term.subst_env σ' t) t h this,
+    have term.subst x v' t = t, from unchanged_of_subst_nonfree_term (t_closed x),
+    show term.subst_env (σ'[x↦v']) t = t, from eq.trans h2 this
+  )
+end
+
 lemma term.subst_env.var {σ: env} {x: var}:
       ((σ x = none) ↔ (term.subst_env σ x = x)) ∧ (∀v, (σ x = some v) ↔ (term.subst_env σ x = v)) :=
 begin
@@ -1553,6 +1721,78 @@ lemma term.not_free_of_subst {x: var} {v: value} {t: term}: x ∉ FV (term.subst
     end
   end
 
+lemma term.not_free_of_substt {x: var} {t₁ t₂: term}: closed t₁ → x ∉ FV (term.substt x t₁ t₂) :=
+  assume t_closed: closed t₁,
+  assume x_free: x ∈ FV (term.substt x t₁ t₂),
+  begin
+    induction t₂ with a,
+
+    show «false», by begin -- term.value
+      unfold term.substt at x_free,
+      cases x_free
+    end,
+
+    show «false», by begin -- term.var
+      unfold term.substt at x_free,
+      by_cases (x = a) with h,
+      simp[h] at x_free,
+      have : a ∉ FV t₁, from t_closed a,
+      contradiction,
+      simp[h] at x_free,
+      cases x_free,
+      contradiction
+    end,
+
+    show «false», by begin -- term.unop
+      unfold term.substt at x_free,
+      have h, from free_in_term.unop.inv x_free,
+      contradiction
+    end,
+
+    show «false», by begin -- term.binop
+      unfold term.substt at x_free,
+      have h, from free_in_term.binop.inv x_free,
+      cases h with h1 h2,
+      contradiction,
+      contradiction
+    end,
+
+    show «false», by begin -- term.app
+      unfold term.substt at x_free,
+      have h, from free_in_term.app.inv x_free,
+      cases h with h1 h2,
+      contradiction,
+      contradiction
+    end
+  end
+
+lemma term.not_free_of_subst_env {x: var} {σ: env} {t: term}: x ∈ σ → x ∉ FV (term.subst_env σ t) :=
+  assume x_in_σ: x ∈ σ,
+  assume x_free: x ∈ FV (term.subst_env σ t),
+  begin
+    induction σ with σ' y v ih,
+
+    -- env.empty
+    show «false», by cases x_in_σ,
+
+    -- σ'[x↦v]
+    show «false», from (
+      have term.subst_env (σ'[y↦v]) t = term.subst y v (term.subst_env σ' t), by unfold term.subst_env,
+      have x ∈ FV (term.subst y v (term.subst_env σ' t)), from this ▸ x_free,
+      have x_neq_y: x ≠ y, from (free_of_subst_term this).left,
+      have h: x ∈ FV (term.subst_env σ' t), from (free_of_subst_term this).right,
+      have x = y ∨ x ∈ σ', from env.contains.inv x_in_σ,
+      or.elim this (
+        assume : x = y,
+        show «false», from x_neq_y this
+      ) (
+        assume : x ∈ σ',
+        have x ∉ FV (term.subst_env σ' t), from ih this,
+        show «false», from this h
+      )
+    )
+  end
+
 lemma prop.not_free_of_subst {x: var} {v: value} {P: prop}: x ∉ FV (prop.subst x v P) :=
   assume x_free: x ∈ FV (prop.subst x v P),
   begin
@@ -1685,6 +1925,18 @@ lemma prop.not_free_of_subst_env {x: var} {σ: env} {P: prop}: x ∈ σ → x �
     )
   end
 
+lemma term.closed_of_closed_subst {σ: env} {t: term}: closed_subst σ t → closed (term.subst_env σ t) :=
+  assume t_closed_subst: closed_subst σ t,
+  show closed (term.subst_env σ t), from (
+    assume x: var,
+    assume h1: x ∈ FV (term.subst_env σ t),
+    have x ∈ FV t, from (free_of_subst_env_term h1).left,
+    have x ∈ σ.dom, from t_closed_subst this,
+    have x ∈ σ, from this,
+    have h2: x ∉ FV (term.subst_env σ t), from term.not_free_of_subst_env this,
+    show «false», from h2 h1
+  )
+
 lemma prop.closed_of_closed_subst {σ: env} {P: prop}: closed_subst σ P → closed (prop.subst_env σ P) :=
   assume P_closed_subst: closed_subst σ P,
   show closed (prop.subst_env σ P), from (
@@ -1784,6 +2036,294 @@ lemma vc.not_free_of_subst {x: var} {v: value} {P: vc}: x ∉ FV (vc.subst x v P
       have x ∈ FV (P₁.subst x v), from (free_in_vc.univ.inv this).right,
       show «false», from P₁_ih this
     )}
+  end
+
+lemma vc.not_free_of_substt {x: var} {t: term} {P: vc}: closed t → x ∉ FV (vc.substt x t P) :=
+  assume t_closed: closed t,
+  assume x_free: x ∈ FV (vc.substt x t P),
+  begin
+    induction P,
+    case vc.term t₂ { from (
+      have vc.substt x t (vc.term t₂) = (term.substt x t t₂), by unfold vc.substt,
+      have free_in_vc x (vc.term (term.substt x t t₂)), from this ▸ x_free,
+      have x ∈ FV (term.substt x t t₂), from free_in_vc.term.inv this,
+      show «false», from term.not_free_of_substt t_closed this
+    )},
+    case vc.not P₁ P₁_ih { from (
+      have vc.substt x t (vc.not P₁) = (P₁.substt x t).not, by unfold vc.substt,
+      have x ∈ FV (P₁.substt x t).not, from this ▸ x_free,
+      have x ∈ FV (P₁.substt x t), from free_in_vc.not.inv this,
+      show «false», from P₁_ih this
+    )},
+    case vc.and P₁ P₂ P₁_ih P₂_ih { from (
+      have vc.substt x t (vc.and P₁ P₂) = (P₁.substt x t ⋀ P₂.substt x t), by unfold vc.substt,
+      have x ∈ FV (P₁.substt x t ⋀ P₂.substt x t), from this ▸ x_free,
+      or.elim (free_in_vc.and.inv this) (
+        assume : x ∈ FV (P₁.substt x t),
+        show «false», from P₁_ih this
+      ) (
+        assume : x ∈ FV (P₂.substt x t),
+        show «false», from P₂_ih this
+      )
+    )},
+    case vc.or P₁ P₂ P₁_ih P₂_ih { from (
+      have vc.substt x t (vc.or P₁ P₂) = (P₁.substt x t ⋁ P₂.substt x t), by unfold vc.substt,
+      have x ∈ FV (P₁.substt x t ⋁ P₂.substt x t), from this ▸ x_free,
+      or.elim (free_in_vc.or.inv this) (
+        assume : x ∈ FV (P₁.substt x t),
+        show «false», from P₁_ih this
+      ) (
+        assume : x ∈ FV (P₂.substt x t),
+        show «false», from P₂_ih this
+      )
+    )},
+    case vc.pre t₁ t₂ { from (
+      have vc.substt x t (vc.pre t₁ t₂) = vc.pre (term.substt x t t₁) (term.substt x t t₂), by unfold vc.substt,
+      have x ∈ FV (vc.pre (term.substt x t t₁) (term.substt x t t₂)), from this ▸ x_free,
+      or.elim (free_in_vc.pre.inv this) (
+        assume : x ∈ FV (term.substt x t t₁),
+        show «false», from term.not_free_of_substt t_closed this
+      ) (
+        assume : x ∈ FV (term.substt x t t₂),
+        show «false», from term.not_free_of_substt t_closed this
+      )
+    )},
+    case vc.pre₁ op t₁ { from (
+      have vc.substt x t (vc.pre₁ op t₁) = vc.pre₁ op (term.substt x t t₁), by unfold vc.substt,
+      have x ∈ FV (vc.pre₁ op (term.substt x t t₁)), from this ▸ x_free,
+      have x ∈ FV (term.substt x t t₁), from free_in_vc.pre₁.inv this,
+      show «false», from term.not_free_of_substt t_closed this
+    )},
+    case vc.pre₂ op t₁ t₂ { from (
+      have vc.substt x t (vc.pre₂ op t₁ t₂) = vc.pre₂ op (term.substt x t t₁) (term.substt x t t₂),
+      by unfold vc.substt,
+      have x ∈ FV (vc.pre₂ op (term.substt x t t₁) (term.substt x t t₂)), from this ▸ x_free,
+      or.elim (free_in_vc.pre₂.inv this) (
+        assume : x ∈ FV (term.substt x t t₁),
+        show «false», from term.not_free_of_substt t_closed this
+      ) (
+        assume : x ∈ FV (term.substt x t t₂),
+        show «false», from term.not_free_of_substt t_closed this
+      )
+    )},
+    case vc.post t₁ t₂ { from (
+      have vc.substt x t (vc.post t₁ t₂) = vc.post (term.substt x t t₁) (term.substt x t t₂),
+      by unfold vc.substt,
+      have x ∈ FV (vc.post (term.substt x t t₁) (term.substt x t t₂)), from this ▸ x_free,
+      or.elim (free_in_vc.post.inv this) (
+        assume : x ∈ FV (term.substt x t t₁),
+        show «false», from term.not_free_of_substt t_closed this
+      ) (
+        assume : x ∈ FV (term.substt x t t₂),
+        show «false», from term.not_free_of_substt t_closed this
+      )
+    )},
+    case vc.univ y P₁ P₁_ih { from (
+      have vc.substt x t (vc.univ y P₁)
+         = vc.univ y (if x = y then P₁ else P₁.substt x t), by unfold vc.substt,
+      have x ∈ FV (vc.univ y (if x = y then P₁ else P₁.substt x t)), from this ▸ x_free,
+      have y_neq_x: x ≠ y, from (free_in_vc.univ.inv this).left,
+      have x ∈ FV (vc.univ y (P₁.substt x t)), by { simp[y_neq_x] at this, from this },
+      have x ∈ FV (P₁.substt x t), from (free_in_vc.univ.inv this).right,
+      show «false», from P₁_ih this
+    )}
+  end
+
+-- lemma term.not_free_of_substte {x: var} {t₁ t₂: term} {σ: env}:
+--       closed_subst σ t₁ → x ∉ FV (term.substt x (term.subst_env σ t₁) t₂) :=
+--   begin
+--     assume t_closed: closed_subst σ t₁,
+--     assume x_free: x ∈ FV (term.substt x (term.subst_env σ t₁) t₂),
+--     have h1: closed (term.subst_env σ t₁), from term.closed_of_closed_subst t_closed,
+--     have h2: x ∉ FV (term.substt x (term.subst_env σ t₁) t₂), from term.not_free_of_substt h1,
+--     show «false», from h2 x_free
+--   end
+
+lemma term.not_free_of_substte {x: var} {t₁ t₂: term} {σ₁ σ₂: env}:
+      closed_subst σ₁ t₁ → x ∉ FV (term.substt x (term.subst_env σ₂ t₁) t₂) - (σ₁.dom - σ₂.dom) :=
+  begin
+    assume t_closed: closed_subst σ₁ t₁,
+    assume x_free: x ∈ FV (term.substt x (term.subst_env σ₂ t₁) t₂) - (σ₁.dom - σ₂.dom),
+    have h1, from set.mem_of_mem_diff x_free,
+    have h2: x ∈ FV (term.subst_env σ₂ t₁), from free_of_substt_same_term h1,
+    have h3: x ∈ FV t₁ ∧ x ∉ σ₂, from free_of_subst_env_term h2,
+    have h4: x ∈ σ₁, from t_closed h3.left,
+    have h5: x ∉ σ₂, from h3.right,
+    have h6, from set.not_mem_of_mem_diff x_free,
+    have h7, from set.not_mem_or_mem_of_not_mem_diff h6,
+    cases h7,
+    contradiction,
+    contradiction
+  end
+
+lemma vc.not_free_of_substte_step {σ₁: env} {x: var} {t: term} {P: vc}:
+      closed_subst σ₁ t → ∀σ₂, x ∉ FV (vc.substte x t P σ₂) - (σ₁.dom - σ₂.dom) :=
+  begin
+    assume t_closed: closed_subst σ₁ t,
+    induction P,
+    case vc.term t₂ {
+      assume σ₂,
+      assume x_free: x ∈ FV (vc.substte x t (vc.term t₂) σ₂) - (σ₁.dom - σ₂.dom),
+      have h1, from set.mem_of_mem_diff x_free,
+      have h2, from set.not_mem_of_mem_diff x_free,
+      have : (vc.substte x t (vc.term t₂) σ₂ = (term.substt x (term.subst_env σ₂ t) t₂)), by unfold vc.substte,
+      have : free_in_vc x (vc.term (term.substt x (term.subst_env σ₂ t) t₂)), from this ▸ h1,
+      have h3: x ∈ FV (term.substt x (term.subst_env σ₂ t) t₂), from free_in_vc.term.inv this,
+      have : x ∈ FV (term.substt x (term.subst_env σ₂ t) t₂) - (σ₁.dom - σ₂.dom), from set.mem_diff h3 h2, 
+      from term.not_free_of_substte t_closed this
+    },
+    case vc.not P₁ P₁_ih {
+      assume σ₂,
+      assume x_free: x ∈ FV (vc.substte x t P₁.not σ₂) - (σ₁.dom - σ₂.dom),
+      have h1, from set.mem_of_mem_diff x_free,
+      have : (vc.substte x t (vc.not P₁) σ₂ = (P₁.substte x t σ₂).not), by unfold vc.substte,
+      have : x ∈ FV (P₁.substte x t σ₂).not, from this ▸ h1,
+      have h2: x ∈ FV (P₁.substte x t σ₂), from free_in_vc.not.inv this,
+      have h3, from set.not_mem_of_mem_diff x_free,
+      have : x ∈ FV (vc.substte x t P₁ σ₂) - (env.dom σ₁ - env.dom σ₂), from set.mem_diff h2 h3,
+      from P₁_ih σ₂ this
+    },
+    case vc.and P₁ P₂ P₁_ih P₂_ih {
+      assume σ₂,
+      assume x_free: x ∈ FV (vc.substte x t (P₁ ⋀ P₂) σ₂) - (σ₁.dom - σ₂.dom),
+      have h1, from set.mem_of_mem_diff x_free,
+      have h2, from set.not_mem_of_mem_diff x_free,
+      have : (vc.substte x t (vc.and P₁ P₂) σ₂ = (P₁.substte x t σ₂ ⋀ P₂.substte x t σ₂)), by unfold vc.substte,
+      have : x ∈ FV (P₁.substte x t σ₂ ⋀ P₂.substte x t σ₂), from this ▸ h1,
+      from or.elim (free_in_vc.and.inv this) (
+        assume : x ∈ FV (P₁.substte x t σ₂),
+        have x ∈ FV (vc.substte x t P₁ σ₂) - (env.dom σ₁ - env.dom σ₂), from set.mem_diff this h2,
+        show «false», from P₁_ih σ₂ this
+      ) (
+        assume : x ∈ FV (P₂.substte x t σ₂),
+        have x ∈ FV (vc.substte x t P₂ σ₂) - (env.dom σ₁ - env.dom σ₂), from set.mem_diff this h2,
+        show «false», from P₂_ih σ₂ this
+      )
+    },
+    case vc.or P₁ P₂ P₁_ih P₂_ih {
+      assume σ₂,
+      assume x_free: x ∈ FV (vc.substte x t (P₁ ⋁ P₂) σ₂) - (σ₁.dom - σ₂.dom),
+      have h1, from set.mem_of_mem_diff x_free,
+      have h2, from set.not_mem_of_mem_diff x_free,
+      have : (vc.substte x t (vc.or P₁ P₂) σ₂ = (P₁.substte x t σ₂ ⋁ P₂.substte x t σ₂)), by unfold vc.substte,
+      have : x ∈ FV (P₁.substte x t σ₂ ⋁ P₂.substte x t σ₂), from this ▸ h1,
+      from or.elim (free_in_vc.or.inv this) (
+        assume : x ∈ FV (P₁.substte x t σ₂),
+        have x ∈ FV (vc.substte x t P₁ σ₂) - (env.dom σ₁ - env.dom σ₂), from set.mem_diff this h2,
+        show «false», from P₁_ih σ₂ this
+      ) (
+        assume : x ∈ FV (P₂.substte x t σ₂),
+        have x ∈ FV (vc.substte x t P₂ σ₂) - (env.dom σ₁ - env.dom σ₂), from set.mem_diff this h2,
+        show «false», from P₂_ih σ₂ this
+      )
+    },
+    case vc.pre t₁ t₂ {
+      assume σ₂,
+      assume x_free: x ∈ FV (vc.substte x t (vc.pre t₁ t₂) σ₂) - (σ₁.dom - σ₂.dom),
+      have h1, from set.mem_of_mem_diff x_free,
+      have h2, from set.not_mem_of_mem_diff x_free,
+      have : (vc.substte x t (vc.pre t₁ t₂) σ₂
+            = vc.pre (term.substt x (term.subst_env σ₂ t) t₁) (term.substt x (term.subst_env σ₂ t) t₂)),
+      by unfold vc.substte,
+      have : x ∈ FV (vc.pre (term.substt x (term.subst_env σ₂ t) t₁) (term.substt x (term.subst_env σ₂ t) t₂)),
+      from this ▸ h1,
+      from or.elim (free_in_vc.pre.inv this) (
+        assume : x ∈ FV (term.substt x (term.subst_env σ₂ t) t₁),
+        have x ∈ FV (term.substt x (term.subst_env σ₂ t) t₁) - (σ₁.dom - σ₂.dom), from set.mem_diff this h2, 
+        term.not_free_of_substte t_closed this
+      ) (
+        assume : x ∈ FV (term.substt x (term.subst_env σ₂ t) t₂),
+        have x ∈ FV (term.substt x (term.subst_env σ₂ t) t₂) - (σ₁.dom - σ₂.dom), from set.mem_diff this h2, 
+        term.not_free_of_substte t_closed this
+      )
+    },
+    case vc.pre₁ op t₁ {
+      assume σ₂,
+      assume x_free: x ∈ FV (vc.substte x t (vc.pre₁ op t₁) σ₂) - (σ₁.dom - σ₂.dom),
+      have h1, from set.mem_of_mem_diff x_free,
+      have h2, from set.not_mem_of_mem_diff x_free,
+      have : (vc.substte x t (vc.pre₁ op t₁) σ₂ = vc.pre₁ op (term.substt x (term.subst_env σ₂ t) t₁)),
+      by unfold vc.substte,
+      have : x ∈ FV (vc.pre₁ op (term.substt x (term.subst_env σ₂ t) t₁)), from this ▸ h1,
+      have : x ∈ FV (term.substt x (term.subst_env σ₂ t) t₁), from free_in_vc.pre₁.inv this,
+      have : x ∈ FV (term.substt x (term.subst_env σ₂ t) t₁) - (σ₁.dom - σ₂.dom), from set.mem_diff this h2, 
+      from term.not_free_of_substte t_closed this
+    },
+    case vc.pre₂ op t₁ t₂ {
+      assume σ₂,
+      assume x_free: x ∈ FV (vc.substte x t (vc.pre₂ op t₁ t₂) σ₂) - (σ₁.dom - σ₂.dom),
+      have h1, from set.mem_of_mem_diff x_free,
+      have h2, from set.not_mem_of_mem_diff x_free,
+      have : (vc.substte x t (vc.pre₂ op t₁ t₂) σ₂
+            = vc.pre₂ op (term.substt x (term.subst_env σ₂ t) t₁) (term.substt x (term.subst_env σ₂ t) t₂)),
+      by unfold vc.substte,
+      have : x ∈ FV (vc.pre₂ op (term.substt x (term.subst_env σ₂ t) t₁) (term.substt x (term.subst_env σ₂ t) t₂)),
+      from this ▸ h1,
+      from or.elim (free_in_vc.pre₂.inv this) (
+        assume : x ∈ FV (term.substt x (term.subst_env σ₂ t) t₁),
+        have x ∈ FV (term.substt x (term.subst_env σ₂ t) t₁) - (σ₁.dom - σ₂.dom), from set.mem_diff this h2, 
+        term.not_free_of_substte t_closed this
+      ) (
+        assume : x ∈ FV (term.substt x (term.subst_env σ₂ t) t₂),
+        have x ∈ FV (term.substt x (term.subst_env σ₂ t) t₂) - (σ₁.dom - σ₂.dom), from set.mem_diff this h2, 
+        term.not_free_of_substte t_closed this
+      )
+    },
+    case vc.post t₁ t₂ {
+      assume σ₂,
+      assume x_free: x ∈ FV (vc.substte x t (vc.post t₁ t₂) σ₂) - (σ₁.dom - σ₂.dom),
+      have h1, from set.mem_of_mem_diff x_free,
+      have h2, from set.not_mem_of_mem_diff x_free,
+      have : (vc.substte x t (vc.post t₁ t₂) σ₂
+            = vc.post (term.substt x (term.subst_env σ₂ t) t₁) (term.substt x (term.subst_env σ₂ t) t₂)),
+      by unfold vc.substte,
+      have : x ∈ FV (vc.post (term.substt x (term.subst_env σ₂ t) t₁) (term.substt x (term.subst_env σ₂ t) t₂)),
+      from this ▸ h1,
+      from or.elim (free_in_vc.post.inv this) (
+        assume : x ∈ FV (term.substt x (term.subst_env σ₂ t) t₁),
+        have x ∈ FV (term.substt x (term.subst_env σ₂ t) t₁) - (σ₁.dom - σ₂.dom), from set.mem_diff this h2, 
+        term.not_free_of_substte t_closed this
+      ) (
+        assume : x ∈ FV (term.substt x (term.subst_env σ₂ t) t₂),
+        have x ∈ FV (term.substt x (term.subst_env σ₂ t) t₂) - (σ₁.dom - σ₂.dom), from set.mem_diff this h2, 
+        term.not_free_of_substte t_closed this
+      )
+    },
+    case vc.univ y P₁ P₁_ih {
+      assume σ₂,
+      assume x_free: x ∈ FV (vc.substte x t (vc.univ y P₁) σ₂) - (σ₁.dom - σ₂.dom),
+      have h1, from set.mem_of_mem_diff x_free,
+      have h2, from set.not_mem_of_mem_diff x_free,
+      have : (vc.substte x t (vc.univ y P₁) σ₂ = vc.univ y (if x = y then P₁ else P₁.substte x t (σ₂.without y))),
+      by unfold vc.substte,
+      have : x ∈ FV (vc.univ y (if x = y then P₁ else P₁.substte x t (σ₂.without y))), from this ▸ h1,
+      have y_neq_x: x ≠ y, from (free_in_vc.univ.inv this).left,
+      have : x ∈ FV (vc.univ y (P₁.substte x t (σ₂.without y))), by { simp[y_neq_x] at this, from this },
+      have h3: x ∈ FV (P₁.substte x t (σ₂.without y)), from (free_in_vc.univ.inv this).right,
+      have h4: x ∉ σ₁.dom - (σ₂.without y).dom, by begin
+        assume h5: x ∈ env.dom σ₁ - env.dom (env.without σ₂ y),
+        have h6, from set.mem_of_mem_diff h5,
+        have h7, from set.not_mem_of_mem_diff h5,
+        have h8, from set.not_mem_or_mem_of_not_mem_diff h2,
+        cases h8 with h9 h10,
+        contradiction,
+        have : x ∈ σ₂.without y, from env.contains_without.rinv ⟨h10, y_neq_x⟩,
+        contradiction
+      end,
+      have : x ∈ FV (vc.substte x t P₁ (σ₂.without y)) - (env.dom σ₁ - env.dom (σ₂.without y)),
+      from set.mem_diff h3 h4,
+      show «false», from P₁_ih (σ₂.without y) this
+    }
+  end
+
+lemma vc.not_free_of_substte {σ: env} {x: var} {t: term} {P: vc}:
+      closed_subst σ t → x ∉ FV (vc.substte x t P σ) :=
+  begin
+    assume t_closed: closed_subst σ t,
+    have : x ∉ FV (vc.substte x t P σ) \ (σ.dom - σ.dom), from vc.not_free_of_substte_step t_closed σ,
+    rw[set.diff_self] at this,
+    rw[set.diff_empty] at this,
+    from this
   end
 
 lemma vc.not_free_of_subst_env {x: var} {σ: env} {P: vc}: x ∈ σ → x ∉ FV (vc.subst_env σ P) :=
@@ -2072,6 +2612,16 @@ lemma term.free_of_free_in_subst {x y: var} {v: value} {t: term}: x ∈ FV (term
       from t₅_ih a
     end
   end
+
+lemma term.closed_subst_of_closed {σ: env} {t: term}: closed (term.subst_env σ t) → closed_subst σ t :=
+  assume t_closed_subst: closed (term.subst_env σ t),
+  show closed_subst σ t, from (
+    assume x: var,
+    assume h1: x ∈ FV t,
+    have ¬ x ∉ σ, from mt (term.free_of_subst_env h1) (t_closed_subst x),
+    have x ∈ σ, from of_not_not this,
+    show x ∈ σ.dom, from this
+  )
 
 lemma prop.free_of_free_in_subst {x y: var} {v: value} {P: prop}: x ∈ FV (prop.subst y v P) → x ∈ FV P :=
   begin
@@ -3050,6 +3600,15 @@ lemma vc.closed_subst.implies {P Q: vc} {σ: env}:
   assume Q_closed_subst: closed_subst σ Q,
   show closed_subst σ (P.not ⋁ Q), from vc.closed_subst.or P_not_closed_subst Q_closed_subst
 
+lemma vc.closed_subst.term.inv {t: term} {σ: env}: closed_subst σ (vc.term t) → closed_subst σ t :=
+  assume t_closed: closed_subst σ (vc.term t),
+  show closed_subst σ t, from (
+    assume x: var,
+    assume : x ∈ FV t,
+    have free_in_vc x (vc.term t), from free_in_vc.term this,
+    show x ∈ σ.dom, from t_closed this
+  )
+
 lemma vc.closed_subst.and.inv {P Q: vc} {σ: env}: closed_subst σ (P ⋀ Q) → (closed_subst σ P ∧ closed_subst σ Q) :=
   assume P_and_Q_closed_subst: closed_subst σ (P ⋀ Q),
   have P_closed_subst: closed_subst σ P, from (
@@ -3136,3 +3695,1288 @@ lemma subst_closed_of_forall_closed {P: prop} {σ: env} {x: var} {v: value}:
     have y ∈ FV (prop.forallc x P), from free_in_prop.forallc this.left this.right,
     show y ∈ σ, from h1 this
   )
+
+lemma contains_of_free_in_nonempty_env {σ: env} {x y: var} {v: value}: (x ≠ y → y ∈ σ) → y ∈ (σ[x↦v]) :=
+  assume ih: x ≠ y → y ∈ σ,
+  if x_eq_y: x = y ∧ option.is_none (σ.apply y) then (
+    have h: σ[x↦v].apply x = (if x = x ∧ option.is_none (σ.apply x) then ↑v else σ.apply x), by unfold env.apply,
+    have (if x = x ∧ option.is_none (σ.apply x) then ↑v else σ.apply x) = ↑v, by simp [x_eq_y],
+    have σ[x↦v].apply x = ↑v, from eq.trans h this,
+    have σ[x↦v].apply y = some v, from x_eq_y.left ▸ this,
+    have ∃v', σ[x↦v] y = some v', from exists.intro v this,
+    show y ∈ (σ[x↦v]), from env.contains_apply_equiv.right.mp this
+  ) else (
+    have y ∈ σ, from (
+      have ¬(x = y) ∨ ¬(option.is_none (σ.apply y)), from not_and_distrib.mp x_eq_y,
+      this.elim (
+        assume : x ≠ y,
+        show y ∈ σ, from ih this        
+      ) ( 
+        assume : ¬(option.is_none (env.apply σ y)),
+        have ¬(option.is_none (σ y)), from this,
+        have option.is_some (σ y), from option.some_iff_not_none.mpr this,
+        have ∃v', σ y = some v', from option.is_some_iff_exists.mp this,
+        show y ∈ σ, from env.contains_apply_equiv.right.mp this
+      )
+    ),
+    let ⟨v', σ_has_y⟩ := (env.contains_apply_equiv.right.mpr this) in
+    have h: σ[x↦v].apply y = (if x = y ∧ option.is_none (σ.apply y) then ↑v else σ.apply y), by unfold env.apply,
+    have (if x = y ∧ option.is_none (σ.apply y) then ↑v else σ.apply y) = σ.apply y, by simp *,
+    have σ[x↦v].apply y = σ.apply y, from this ▸ h,
+    have σ[x↦v].apply y = some v', from eq.trans this σ_has_y,
+    have ∃v', σ[x↦v] y = some v', from exists.intro v' this,
+    show y ∈ (σ[x↦v]), from env.contains_apply_equiv.right.mp this
+  )
+
+lemma contains_of_free_eq_value {P: prop} {σ: env} {x y: var} {v: value}:
+  x ∈ FV (P ⋀ (y ≡ v)) → (x ∈ FV P → x ∈ σ) → x ∈ (σ[y↦v]) :=
+  assume x_free_in_P: x ∈ FV (P ⋀ (y ≡ v)),
+  assume ih : x ∈ FV P → x ∈ σ,
+  contains_of_free_in_nonempty_env (
+    assume x'_is_not_x: y ≠ x,
+    have free_in_prop x P ∨ free_in_prop x (y ≡ v), from free_in_prop.and.inv x_free_in_P,
+    or.elim this (
+      assume x_free_in_P: free_in_prop x P,
+      show x ∈ σ, from ih x_free_in_P
+    ) (
+      assume x_free_in_eq_v: free_in_prop x (y ≡ v),
+      show x ∈ σ, by begin
+        cases x_free_in_eq_v,
+        case free_in_prop.term x_free_in_eq {
+          cases x_free_in_eq,
+          case free_in_term.binop₁ free_in_y {
+            have y_is_x: (y = x), from (free_in_term.var.inv free_in_y).symm,
+            contradiction
+          },
+          case free_in_term.binop₂ free_in_v {
+            cases free_in_v
+          }
+        }
+      end
+    )
+  )
+
+lemma env.dom.inv {σ: env} {x: var} {v: value}: (σ[x↦v]).dom = (σ.dom ∪ set.insert x ∅) :=
+  set.eq_of_subset_of_subset (
+    assume y: var,
+    assume : y ∈ (σ[x↦v]).dom,
+    have y ∈ (σ[x↦v]), from this,
+    or.elim (env.contains.inv this) (
+      assume : y = x,
+      have y ∈ set.insert x ∅, from set.mem_singleton_of_eq this,
+      show y ∈ (σ.dom ∪ set.insert x ∅), from set.mem_union_right σ.dom this
+    ) (
+      assume : y ∈ σ,
+      have y ∈ σ.dom, from this,
+      show y ∈ (σ.dom ∪ set.insert x ∅), from set.mem_union_left (set.insert x ∅) this
+    )
+  ) (
+    assume y: var,
+    assume : y ∈ (σ.dom ∪ set.insert x ∅),
+    or.elim (set.mem_or_mem_of_mem_union this) (
+      assume : y ∈ σ.dom,
+      have y ∈ σ, from this,
+      have y ∈ (σ[x↦v]), from env.contains.rest this,
+      show y ∈ (σ[x↦v]).dom, from this
+    ) (
+      assume : y ∈ set.insert x ∅,
+      have y = x, from (set.mem_singleton_iff y x).mp this,
+      have y ∈ (σ[x↦v]), from this ▸ env.contains.same,
+      show y ∈ (σ[x↦v]).dom, from this
+    )
+  )
+
+lemma env.dom.two_elems {σ: env} {x y: var} {v₁ v₂: value}: (σ[x↦v₁][y↦v₂]).dom = σ.dom ∪ {x, y} :=
+  by calc (σ[x↦v₁][y↦v₂]).dom = (σ[x↦v₁]).dom ∪ set.insert y ∅ : env.dom.inv
+                           ... = σ.dom ∪ set.insert x ∅ ∪ set.insert y ∅ : by rw[env.dom.inv]
+                           ... = σ.dom ∪ (set.insert x ∅ ∪ set.insert y ∅) : by rw[set.union_assoc]
+                           ... = σ.dom ∪ {x, y} : by rw[set.two_elems_of_insert]
+
+lemma env.apply_of_contains {σ: env} {x: var} {v: value}: x ∉ σ → ((σ[x↦v]) x = v) :=
+  begin
+    intro h,
+    change (env.apply (σ[x↦v]) x = some v),
+    unfold env.apply,
+    by_cases (x = x ∧ (option.is_none (env.apply σ x))) with h2,
+    simp[h2],
+    refl,
+    simp at h2,
+    have h3, from env.contains_apply_equiv.left.mpr h,
+    have h4: (env.apply σ x = none), from h3,
+    rw[h4] at h2,
+    unfold option.is_none at h2,
+    have h5: (↑tt = «false»), from eq_false_intro h2,
+    have h6: (↑tt = «true»), by simp,
+    have h7: («false» = «true»), from eq.trans h5.symm h6,
+    have h8: «true», from trivial,
+    have r9: «false», from h7.symm ▸ h8,
+    contradiction
+  end
+
+lemma env.equiv_of_rest_and_same {σ σ': env} {x: var} {v: value}:
+      (∀y, y ∈ σ → (σ y = σ' y)) → x ∉ σ → (σ' x = v) → (∀y, y ∈ (σ[x↦v]) → ((σ[x↦v]) y = σ' y)) :=
+  assume h1: (∀y, y ∈ σ → (σ y = σ' y)),
+  assume h2: x ∉ σ,
+  assume h3: σ' x = v,
+  assume y: var,
+  assume h4: y ∈ (σ[x↦v]),
+  if h: x = y then (
+    have h5: (σ[x↦v]) y = v, from h ▸ env.apply_of_contains h2,
+    show ((σ[x↦v]) y = σ' y), from eq.trans h5 (h ▸ h3.symm)
+  ) else (
+    have y ∈ σ, from (
+      have y = x ∨ y ∈ σ, from env.contains.inv h4,
+      or.elim this.symm id (
+        assume : y = x,
+        show y ∈ σ, from absurd this.symm h
+      )
+    ),
+    have h6: σ y = σ' y, from h1 y this,
+    have env.apply (σ[x↦v]) y = σ.apply y, by { unfold env.apply, simp[h] },
+    have (σ[x↦v]) y = σ y, from this,
+    show ((σ[x↦v]) y = σ' y), from this.symm ▸ h6
+  )
+
+lemma env.equiv_of_not_contains {σ σ': env} {x: var} {v: value}:
+      (∀y, y ∈ σ → (σ y = σ' y)) → x ∉ σ → (∀y, y ∈ σ → (σ y = (σ'[x↦v]) y)) :=
+  assume h1: (∀y, y ∈ σ → (σ y = σ' y)),
+  assume h2: x ∉ σ,
+  assume y: var,
+  assume h4: y ∈ σ,
+  if h: x = y then (
+    have x ∈ σ, from h.symm ▸ h4,
+    show σ y = (σ'[x↦v]) y, from absurd this h2
+  ) else (
+    have h2: σ y = σ' y, from h1 y h4,
+    have (∃v, σ y = some v), from env.contains_apply_equiv.right.mpr h4,
+    have option.is_some (σ y), from option.is_some_iff_exists.mpr this,
+    have ¬ option.is_none (σ y), from option.some_iff_not_none.mp this,
+    have h5: ¬ (x = y ∧ option.is_none (env.apply σ' y)), from not_and_distrib.mpr (or.inl h),
+    have env.apply (σ'[x↦v]) y = σ' y, by { unfold env.apply, simp[h5], refl },
+    show σ y = (σ'[x↦v]) y, from eq.trans h2 this.symm
+  )
+
+lemma env.apply_of_rest_apply {σ: env} {x y: var} {vx vy: value}:
+      (σ x = vx) → ((σ[y↦vy]) x = vx) :=
+  begin
+    assume h1: (env.apply σ x = some vx),
+    change (env.apply (σ[y↦vy]) x = ↑vx),
+    unfold env.apply,
+    have h2, from option.is_some_iff_exists.mpr (exists.intro vx h1),
+    have h3, from option.some_iff_not_none.mp h2,
+    have h4: ¬ (y = x ∧ (option.is_none (env.apply σ x))),
+    from not_and_distrib.mpr (or.inr h3),
+    simp[h4],
+    from h1
+  end
+
+lemma term.subst_env.order {t: term} {σ: env} {x: var} {v: value}:
+      (x ∉ σ) ∨ (σ x = v) → (term.subst_env σ (term.subst x v t) = term.subst x v (term.subst_env σ t)) :=
+  begin
+    assume h1,
+    induction t with v' y unop t₁ t₁_ih binop t₂ t₃ t₂_ih t₃_ih t₄ t₅ t₄_ih t₅_ih,
+    
+    show (term.subst_env σ (term.subst x v (term.value v')) = term.subst x v (term.subst_env σ (term.value v'))),
+    by begin
+      change (term.subst_env σ (term.subst x v (term.value v')) = term.subst x v (term.subst_env σ v')),
+      rw[term.subst_env.value],
+      unfold term.subst,
+      rw[term.subst_env.value],
+      change (↑v' = term.subst x v (term.value v')),
+      unfold term.subst
+    end,
+
+    show (term.subst_env σ (term.subst x v (term.var y)) = term.subst x v (term.subst_env σ (term.var y))),
+    by begin
+      by_cases (x = y) with h,
+      simp[h],
+      rw[h] at h1,
+      unfold term.subst,
+      simp,
+      cases h1,
+      have : (σ y = none), from env.contains_apply_equiv.left.mpr a,
+      have h2: (term.subst_env σ (term.var y) = y), from term.subst_env.var.left.mp this,
+      simp[h2],
+      rw[term.subst_env.value],
+      change (↑v = term.subst y v (term.var y)),
+      unfold term.subst,
+      simp,
+
+      have h2: (term.subst_env σ (term.var y) = v), from (term.subst_env.var.right v).mp a,
+      rw[h2],
+      change (term.subst_env σ ↑v = term.subst y v (term.value v)),
+      unfold term.subst,
+      rw[term.subst_env.value],
+
+      have h2: (term.subst x v (term.var y) = y), from term.subst.var.diff h,
+      rw[h2],
+      by_cases (y ∈ σ) with h3,
+      
+      have h4, from env.contains_apply_equiv.right.mpr h3,
+      cases h4 with v' h5,
+      have h6: (term.subst_env σ y = v'), from (term.subst_env.var.right v').mp h5,
+      rw[h6],
+      change (↑v' = term.subst x v (term.subst_env σ ↑y)),
+      rw[h6],
+      change (↑v' = term.subst x v (term.value v')),
+      unfold term.subst,
+
+      have : (σ y = none), from env.contains_apply_equiv.left.mpr h3,
+      have h4: (term.subst_env σ (term.var y) = y), from term.subst_env.var.left.mp this,
+      simp[h4],
+      change (term.subst_env σ (term.var y) = term.subst x v (term.var y)),
+      rw[h2],
+      rw[h4]
+    end,
+
+    show (term.subst_env σ (term.subst x v (term.unop unop t₁))
+        = term.subst x v (term.subst_env σ (term.unop unop t₁))), by begin
+      rw[term.subst_env.unop],
+      unfold term.subst,
+      rw[term.subst_env.unop],
+      congr,
+      from t₁_ih
+    end,
+
+    show (term.subst_env σ (term.subst x v (term.binop binop t₂ t₃))
+        = term.subst x v (term.subst_env σ (term.binop binop t₂ t₃))), by begin
+      rw[term.subst_env.binop],
+      unfold term.subst,
+      rw[term.subst_env.binop],
+      congr,
+      rw[t₂_ih],
+      rw[t₃_ih]
+    end,
+
+    show (term.subst_env σ (term.subst x v (term.app t₄ t₅))
+        = term.subst x v (term.subst_env σ (term.app t₄ t₅))), by begin
+      rw[term.subst_env.app],
+      unfold term.subst,
+      rw[term.subst_env.app],
+      congr,
+      rw[t₄_ih],
+      rw[t₅_ih]
+    end
+  end
+
+lemma term.substt_env.order {t' t: term} {σ: env} {x: var}:
+      closed t' → (x ∉ σ) → (term.subst_env σ (term.substt x t' t) = term.substt x t' (term.subst_env σ t)) :=
+  begin
+    assume t'_closed,
+    assume h1,
+    induction t with v y unop t₁ t₁_ih binop t₂ t₃ t₂_ih t₃_ih t₄ t₅ t₄_ih t₅_ih,
+    
+    show (term.subst_env σ (term.substt x t' (term.value v)) = term.substt x t' (term.subst_env σ (term.value v))),
+    by begin
+      change (term.subst_env σ (term.substt x t' (term.value v)) = term.substt x t' (term.subst_env σ v)),
+      rw[term.subst_env.value],
+      unfold term.substt,
+      rw[term.subst_env.value],
+      change (↑v = term.substt x t' (term.value v)),
+      unfold term.substt
+    end,
+
+    show (term.subst_env σ (term.substt x t' (term.var y)) = term.substt x t' (term.subst_env σ (term.var y))),
+    by begin
+      by_cases (x = y) with h,
+      simp[h],
+      rw[h] at h1,
+      unfold term.substt,
+      simp,
+      have : (σ y = none), from env.contains_apply_equiv.left.mpr h1,
+      have h2: (term.subst_env σ (term.var y) = y), from term.subst_env.var.left.mp this,
+      simp[h2],
+      rw[term.subst_env.closed t'_closed],
+      change (t' = term.substt y t' (term.var y)),
+      unfold term.substt,
+      simp,
+
+      have h2: (term.substt x t' (term.var y) = y), from term.substt.var.diff h,
+      rw[h2],
+      by_cases (y ∈ σ) with h3,
+      
+      have h4, from env.contains_apply_equiv.right.mpr h3,
+      cases h4 with v' h5,
+      have h6: (term.subst_env σ y = v'), from (term.subst_env.var.right v').mp h5,
+      rw[h6],
+      change (↑v' = term.substt x t' (term.subst_env σ ↑y)),
+      rw[h6],
+      change (↑v' = term.substt x t' (term.value v')),
+      unfold term.substt,
+
+      have : (σ y = none), from env.contains_apply_equiv.left.mpr h3,
+      have h4: (term.subst_env σ (term.var y) = y), from term.subst_env.var.left.mp this,
+      simp[h4],
+      change (term.subst_env σ (term.var y) = term.substt x t' (term.var y)),
+      rw[h2],
+      rw[h4]
+    end,
+
+    show (term.subst_env σ (term.substt x t' (term.unop unop t₁))
+        = term.substt x t' (term.subst_env σ (term.unop unop t₁))), by begin
+      rw[term.subst_env.unop],
+      unfold term.substt,
+      rw[term.subst_env.unop],
+      congr,
+      from t₁_ih
+    end,
+
+    show (term.subst_env σ (term.substt x t' (term.binop binop t₂ t₃))
+        = term.substt x t' (term.subst_env σ (term.binop binop t₂ t₃))), by begin
+      rw[term.subst_env.binop],
+      unfold term.substt,
+      rw[term.subst_env.binop],
+      congr,
+      rw[t₂_ih],
+      rw[t₃_ih]
+    end,
+
+    show (term.subst_env σ (term.substt x t' (term.app t₄ t₅))
+        = term.substt x t' (term.subst_env σ (term.app t₄ t₅))), by begin
+      rw[term.subst_env.app],
+      unfold term.substt,
+      rw[term.subst_env.app],
+      congr,
+      rw[t₄_ih],
+      rw[t₅_ih]
+    end
+  end
+
+lemma term.subst_env_inner {t: term} {σ: env} {x: var} {v: value}:
+      (σ x = some v) → (term.subst_env σ (term.subst x v t) = term.subst_env σ t) :=
+  begin
+    assume x_is_v,
+
+    induction σ with σ₁ y v' ih,
+
+    show (term.subst_env env.empty (term.subst x v t) = term.subst_env env.empty t), by cases x_is_v,
+
+    show (term.subst_env (σ₁[y↦v']) (term.subst x v t) = term.subst_env (σ₁[y↦v']) t), by begin
+      unfold term.subst_env,
+      have h2: (env.apply (σ₁[y↦v']) x = some v), from x_is_v,
+      unfold env.apply at h2,
+      by_cases (y = x ∧ (option.is_none (env.apply σ₁ x))) with h3,
+      simp[h3] at h2,
+      have h4: (v' = v), from option.some.inj h2,
+      simp[h3],
+      have h5: (σ₁ x = none), from option.is_none.inv.mpr h3.right,
+      have h6: x ∉ σ₁, from env.contains_apply_equiv.left.mp h5,
+      rw[h4],
+      have h7: x ∉ FV (term.subst x v t), from term.not_free_of_subst,
+      have h8: x ∉ FV (term.subst_env σ₁ (term.subst x v t)),
+      have : ¬(free_in_term x (term.subst x v t) ∧ x ∉ σ₁), by begin
+        assume : free_in_term x (term.subst x v t) ∧ x ∉ σ₁,
+        show «false», from h7 this.left
+      end,
+      from mt free_of_subst_env_term this,
+      have h9: (term.subst x v (term.subst_env σ₁ (term.subst x v t)) = (term.subst_env σ₁ (term.subst x v t))),
+      from unchanged_of_subst_nonfree_term h8,
+      rw[h9],
+      from term.subst_env.order (or.inl h6),
+
+      simp[h3] at h2,
+      have h4, from ih h2,
+      congr,
+      from h4
+    end
+  end
+
+lemma term.subst_env_twice {t: term} {σ: env}:
+  term.subst_env σ (term.subst_env σ t) = term.subst_env σ t :=
+  begin
+    induction σ with σ' x v ih,
+    
+    show (term.subst_env env.empty (term.subst_env env.empty t) = term.subst_env env.empty t), by begin
+      unfold term.subst_env
+    end,
+
+    show (term.subst_env (σ'[x↦v]) (term.subst_env (σ'[x↦v]) t) = term.subst_env (σ'[x↦v]) t), by begin
+
+      by_cases (x ∈ σ') with h1,
+      unfold term.subst_env,
+
+      have h2: x ∉ FV (term.subst_env σ' t), from term.not_free_of_subst_env h1,
+      have h3: (term.subst x v (term.subst_env σ' t) = (term.subst_env σ' t)),
+      from unchanged_of_subst_nonfree_term h2,
+      rw[h3],
+      have h4: x ∉ FV (term.subst_env σ' (term.subst_env σ' t)), from term.not_free_of_subst_env h1,
+      have h5: (term.subst x v (term.subst_env σ' (term.subst_env σ' t)) = (term.subst_env σ' (term.subst_env σ' t))),
+      from unchanged_of_subst_nonfree_term h4,
+      rw[h5],
+      from ih,
+
+      have h6: (term.subst_env (σ'[x↦v]) t = term.subst x v (term.subst_env σ' t)),
+      by unfold term.subst_env,
+      rw[h6],
+
+      have h7: (env.apply (σ'[x↦v]) x = v), from env.apply_of_contains h1,
+      have h8: (term.subst_env (σ'[x↦v]) (term.subst x v (term.subst_env σ' t))
+              = term.subst_env (σ'[x↦v]) (term.subst_env σ' t)),
+      from term.subst_env_inner h7,
+      rw[h8],
+      unfold term.subst_env,
+      congr,
+      from ih
+    end
+  end
+
+lemma env.dom_subset_of_equivalent_env {σ₁ σ₂: env}:
+  (∀z, z ∈ σ₁ → (σ₁ z = σ₂ z)) → (σ₁.dom ⊆ σ₂.dom) :=
+  assume env_equiv: (∀z, z ∈ σ₁ → (σ₁ z = σ₂ z)),
+  assume x: var,
+  assume : x ∈ σ₁.dom,
+  have h1: x ∈ σ₁, from this,
+  have ∃v, σ₁ x = some v, from env.contains_apply_equiv.right.mpr h1,
+  let ⟨v, h2⟩ := this in
+  have σ₁ x = σ₂ x, from env_equiv x h1,
+  have σ₂ x = some v, from eq.trans this.symm h2,
+  show x ∈ σ₂, from env.contains_apply_equiv.right.mp (exists.intro v this)
+
+lemma env.empty_of_dom_empty {σ: env}: (σ.dom = ∅) → (σ = env.empty) :=
+  begin
+    assume h1: (σ.dom = ∅),
+    cases σ with σ' x v,
+    refl,
+    have h2, from set.subset_of_eq h1,
+    have h3: x ∈ (σ'[x↦v]), from env.contains.same,
+    have h4: x ∈ (σ'[x↦v]).dom, from h3,
+    have h5, from set.mem_of_subset_of_mem h2 h4,
+    have : x ∉ ∅, from set.not_mem_empty x,
+    contradiction
+  end
+
+lemma env.empty_dom_is_empty: (env.empty.dom = ∅) :=
+  begin
+    apply set.eq_of_subset_of_subset,
+    assume x: var,
+    assume : x ∈ env.dom env.empty,
+    have h2: x ∈ env.empty, from this,
+    cases h2,
+
+    assume x: var,
+    assume : x ∈ ∅,
+    have : x ∉ ∅, from set.not_mem_empty x,
+    contradiction
+  end
+
+lemma term.subst_env_twice_equiv {t: term} {σ₁ σ₂: env}:
+  (∀z, z ∈ σ₁ → (σ₁ z = σ₂ z)) → (term.subst_env σ₁ (term.subst_env σ₂ t) = term.subst_env σ₂ t) :=
+  begin
+    assume env_equiv: ∀z, z ∈ σ₁ → (σ₁ z = σ₂ z),
+    -- have env_subst: σ₁.dom ⊆ σ₂.dom, from env.dom_subset_of_equivalent_env env_equiv,
+
+    induction σ₁ with σ' x v ih,
+    
+    show (term.subst_env env.empty (term.subst_env σ₂ t) = term.subst_env σ₂ t),
+    by unfold term.subst_env,
+
+    show (term.subst_env (σ'[x↦v]) (term.subst_env σ₂ t) = term.subst_env σ₂ t), by begin
+      unfold term.subst_env,
+      have h1: (∀ (z : var), z ∈ σ' → (σ' z = σ₂ z)), by begin
+        assume z: var,
+        assume h2: z ∈ σ',
+        have h3: (env.apply (σ'[x↦v]) z = σ₂ z), from env_equiv z (env.contains.rest h2),
+        unfold env.apply at h3,
+        have h4, from env.contains_apply_equiv.right.mpr h2,
+        have h5, from option.is_some_iff_exists.mpr h4,
+        have h6, from option.some_iff_not_none.mp h5,
+        have h7, from not_and_of_not_right (x = z) h6,
+        have h8: (ite (x = z ∧ (option.is_none (env.apply σ' z))) ↑v (env.apply σ' z) = (env.apply σ' z)),
+        from ite.if_false h7,
+        rw[h8] at h3,
+        from h3
+      end,
+
+      have h2: (term.subst_env σ' (term.subst_env σ₂ t) = term.subst_env σ₂ t), from ih h1,
+      rw[h2],
+      have h3: x ∈ σ₂, by begin
+        have h3: (env.apply (σ'[x↦v]) x = σ₂ x), from env_equiv x env.contains.same,
+        unfold env.apply at h3,
+        by_cases (x ∈ σ') with h4,
+
+        have h5, from env.contains_apply_equiv.right.mpr h4,
+        have h6, from option.is_some_iff_exists.mpr h5,
+        have h7, from option.some_iff_not_none.mp h6,
+        have h8, from not_and_of_not_right (x = x) h7,
+        have h9: (ite (x = x ∧ (option.is_none (env.apply σ' x))) ↑v (env.apply σ' x) = (env.apply σ' x)),
+        from ite.if_false h8,
+        rw[h9] at h3,
+        have h10: (σ' x = σ₂ x), from h3,
+        rw[h10] at h5,
+        from env.contains_apply_equiv.right.mp h5,
+
+        have h5, from env.contains_apply_equiv.left.mpr h4,
+        have h6, from option.is_none.inv.mp h5,
+        have h7: (ite (x = x ∧ (option.is_none (env.apply σ' x))) ↑v (env.apply σ' x) = v),
+        from ite.if_true ⟨rfl, h6⟩,
+        rw[h7] at h3,
+        from env.contains_apply_equiv.right.mp (exists.intro v h3.symm)
+      end,
+
+      have : x ∉ FV (term.subst_env σ₂ t), from term.not_free_of_subst_env h3,
+      from unchanged_of_subst_nonfree_term this
+    end
+  end
+
+lemma term.substte_env.order {t' t: term} {σ₁ σ₂: env} {x: var}:
+      (∀z, z ∈ σ₁ → (σ₁ z = σ₂ z)) → (x ∉ σ₁) →
+      (term.subst_env σ₁ (term.substt x (term.subst_env σ₂ t') t)
+     = term.substt x (term.subst_env σ₂ t') (term.subst_env σ₁ t)) :=
+  begin
+    assume env_equiv,
+    assume h1,
+    induction t with v y unop t₁ t₁_ih binop t₂ t₃ t₂_ih t₃_ih t₄ t₅ t₄_ih t₅_ih,
+    
+    show (term.subst_env σ₁ (term.substt x (term.subst_env σ₂ t') (term.value v))
+        = term.substt x (term.subst_env σ₂ t') (term.subst_env σ₁ (term.value v))),
+    by begin
+      change (term.subst_env σ₁ (term.substt x (term.subst_env σ₂ t') (term.value v)) =
+              term.substt x (term.subst_env σ₂ t') (term.subst_env σ₁ v)),
+      rw[term.subst_env.value],
+      unfold term.substt,
+      rw[term.subst_env.value],
+      change (↑v = term.substt x (term.subst_env σ₂ t') (term.value v)),
+      unfold term.substt
+    end,
+
+    show (term.subst_env σ₁ (term.substt x (term.subst_env σ₂ t') (term.var y))
+        = term.substt x (term.subst_env σ₂ t') (term.subst_env σ₁ (term.var y))),
+    by begin
+      by_cases (x = y) with h,
+      simp[h],
+      rw[h] at h1,
+      unfold term.substt,
+      simp,
+      have : (σ₁ y = none), from env.contains_apply_equiv.left.mpr h1,
+      have h2: (term.subst_env σ₁ (term.var y) = y), from term.subst_env.var.left.mp this,
+      simp[h2],
+      have h3: (term.subst_env σ₁ (term.subst_env σ₂ t') = (term.subst_env σ₂ t')),
+      from term.subst_env_twice_equiv env_equiv,
+      rw[h3],
+      change (term.subst_env σ₂ t' = term.substt y (term.subst_env σ₂ t') (term.var y)),
+      unfold term.substt,
+      simp,
+
+      unfold term.substt,
+      simp[h],
+      have h3: (term.subst_env σ₁ y = y ∨ ∃v: value, term.subst_env σ₁ y = v),
+      from term.subst_env.var.inv,
+      cases h3 with h4 h5,
+
+      change (term.subst_env σ₁ y = term.substt x (term.subst_env σ₂ t') (term.subst_env σ₁ y)),
+      rw[h4],
+      change (↑y = term.substt x (term.subst_env σ₂ t') (term.var y)),
+      unfold term.substt,
+      simp[h],
+
+      cases h5 with v' h6,
+      change (term.subst_env σ₁ y = term.substt x (term.subst_env σ₂ t') (term.subst_env σ₁ y)),
+      rw[h6],
+      change (↑v' = term.substt x (term.subst_env σ₂ t') (term.value v')),
+      unfold term.substt
+    end,
+
+    show (term.subst_env σ₁ (term.substt x (term.subst_env σ₂ t') (term.unop unop t₁))
+        = term.substt x (term.subst_env σ₂ t') (term.subst_env σ₁ (term.unop unop t₁))), by begin
+      rw[term.subst_env.unop],
+      unfold term.substt,
+      rw[term.subst_env.unop],
+      congr,
+      from t₁_ih
+    end,
+
+    show (term.subst_env σ₁ (term.substt x (term.subst_env σ₂ t') (term.binop binop t₂ t₃))
+        = term.substt x (term.subst_env σ₂ t') (term.subst_env σ₁ (term.binop binop t₂ t₃))), by begin
+      rw[term.subst_env.binop],
+      unfold term.substt,
+      rw[term.subst_env.binop],
+      congr,
+      rw[t₂_ih],
+      rw[t₃_ih]
+    end,
+
+    show (term.subst_env σ₁ (term.substt x (term.subst_env σ₂ t') (term.app t₄ t₅))
+        = term.substt x (term.subst_env σ₂ t') (term.subst_env σ₁ (term.app t₄ t₅))), by begin
+      rw[term.subst_env.app],
+      unfold term.substt,
+      rw[term.subst_env.app],
+      congr,
+      rw[t₄_ih],
+      rw[t₅_ih]
+    end
+  end
+
+lemma vc.subst_env.order {P: vc}:
+    ∀ {σ: env} {x: var} {v: value},
+      (x ∉ σ) ∨ (σ x = v) → (vc.subst_env σ (vc.subst x v P) = vc.subst x v (vc.subst_env σ P)) :=
+  begin
+    induction P,
+    case vc.term t {
+      assume σ x v,
+      assume h1,
+      change (vc.subst_env σ (vc.subst x v (vc.term t)) = vc.subst x v (vc.subst_env σ ↑t)),
+      rw[vc.subst_env.term],
+      unfold vc.subst,
+      rw[vc.subst_env.term],
+      congr,
+      from term.subst_env.order h1
+    },
+    case vc.not P₁ ih {
+      assume σ x v,
+      assume h1,
+      rw[vc.subst_env.not],
+      unfold vc.subst,
+      rw[vc.subst_env.not],
+      congr,
+      from ih h1
+    },
+    case vc.and P₁ P₂ P₁_ih P₂_ih {
+      assume σ x v,
+      assume h1,
+      change (vc.subst_env σ (vc.subst x v (vc.and P₁ P₂)) = vc.subst x v (vc.subst_env σ (P₁ ⋀ P₂))),
+      rw[vc.subst_env.and],
+      unfold vc.subst,
+      rw[vc.subst_env.and],
+      congr,
+      from P₁_ih h1,
+      from P₂_ih h1
+    },
+    case vc.or P₁ P₂ P₁_ih P₂_ih {
+      assume σ x v,
+      assume h1,
+      change (vc.subst_env σ (vc.subst x v (vc.or P₁ P₂)) = vc.subst x v (vc.subst_env σ (P₁ ⋁ P₂))),
+      rw[vc.subst_env.or],
+      unfold vc.subst,
+      rw[vc.subst_env.or],
+      congr,
+      from P₁_ih h1,
+      from P₂_ih h1
+    },
+    case vc.pre t₁ t₂ {
+      assume σ x v,
+      assume h1,
+      rw[vc.subst_env.pre],
+      unfold vc.subst,
+      rw[vc.subst_env.pre],
+      congr,
+      from term.subst_env.order h1,
+      from term.subst_env.order h1
+    },
+    case vc.pre₁ op t {
+      assume σ x v,
+      assume h1,
+      rw[vc.subst_env.pre₁],
+      unfold vc.subst,
+      rw[vc.subst_env.pre₁],
+      congr,
+      from term.subst_env.order h1
+    },
+    case vc.pre₂ op t₁ t₂ {
+      assume σ x v,
+      assume h1,
+      rw[vc.subst_env.pre₂],
+      unfold vc.subst,
+      rw[vc.subst_env.pre₂],
+      congr,
+      from term.subst_env.order h1,
+      from term.subst_env.order h1
+    },
+    case vc.post t₁ t₂ {
+      assume σ x v,
+      assume h1,
+      rw[vc.subst_env.post],
+      unfold vc.subst,
+      rw[vc.subst_env.post],
+      congr,
+      from term.subst_env.order h1,
+      from term.subst_env.order h1
+    },
+    case vc.univ z P' P'_ih {
+      assume σ x v,
+      assume h1,
+      rw[vc.subst_env.univ],
+      unfold vc.subst,
+      by_cases (x = z) with h2,
+
+      simp[h2],
+      rw[vc.subst_env.univ],
+
+      simp[h2],
+      rw[vc.subst_env.univ],
+      congr,
+
+      have h2: (x ∉ σ.without z ∨ (σ.without z x = v)),
+      from env.without_equiv h1,
+      have h3: (vc.subst_env (σ.without z) (vc.subst x v P') = vc.subst x v (vc.subst_env (σ.without z) P')),
+      from P'_ih h2,
+      rw[h3]
+    }
+  end
+
+lemma vc.substt_env.order {P: vc}:
+    ∀ {σ: env} {x: var} {t: term},
+      closed t → (x ∉ σ) → (vc.subst_env σ (vc.substt x t P) = vc.substt x t (vc.subst_env σ P)) :=
+  begin
+    induction P,
+    case vc.term t' {
+      assume σ x t,
+      assume t_closed,
+      assume h1,
+      change (vc.subst_env σ (vc.substt x t (vc.term t')) = vc.substt x t (vc.subst_env σ t')),
+      rw[vc.subst_env.term],
+      unfold vc.substt,
+      rw[vc.subst_env.term],
+      congr,
+      from term.substt_env.order t_closed h1
+    },
+    case vc.not P₁ ih {
+      assume σ x t,
+      assume t_closed,
+      assume h1,
+      rw[vc.subst_env.not],
+      unfold vc.substt,
+      rw[vc.subst_env.not],
+      congr,
+      from ih t_closed h1
+    },
+    case vc.and P₁ P₂ P₁_ih P₂_ih {
+      assume σ x t,
+      assume t_closed,
+      assume h1,
+      change (vc.subst_env σ (vc.substt x t (vc.and P₁ P₂)) = vc.substt x t (vc.subst_env σ (P₁ ⋀ P₂))),
+      rw[vc.subst_env.and],
+      unfold vc.substt,
+      rw[vc.subst_env.and],
+      congr,
+      from P₁_ih t_closed h1,
+      from P₂_ih t_closed h1
+    },
+    case vc.or P₁ P₂ P₁_ih P₂_ih {
+      assume σ x t,
+      assume t_closed,
+      assume h1,
+      change (vc.subst_env σ (vc.substt x t (vc.or P₁ P₂)) = vc.substt x t (vc.subst_env σ (P₁ ⋁ P₂))),
+      rw[vc.subst_env.or],
+      unfold vc.substt,
+      rw[vc.subst_env.or],
+      congr,
+      from P₁_ih t_closed h1,
+      from P₂_ih t_closed h1
+    },
+    case vc.pre t₁ t₂ {
+      assume σ x t,
+      assume t_closed,
+      assume h1,
+      rw[vc.subst_env.pre],
+      unfold vc.substt,
+      rw[vc.subst_env.pre],
+      congr,
+      from term.substt_env.order t_closed h1,
+      from term.substt_env.order t_closed h1
+    },
+    case vc.pre₁ op t {
+      assume σ x t,
+      assume t_closed,
+      assume h1,
+      rw[vc.subst_env.pre₁],
+      unfold vc.substt,
+      rw[vc.subst_env.pre₁],
+      congr,
+      from term.substt_env.order t_closed h1
+    },
+    case vc.pre₂ op t₁ t₂ {
+      assume σ x t,
+      assume t_closed,
+      assume h1,
+      rw[vc.subst_env.pre₂],
+      unfold vc.substt,
+      rw[vc.subst_env.pre₂],
+      congr,
+      from term.substt_env.order t_closed h1,
+      from term.substt_env.order t_closed h1
+    },
+    case vc.post t₁ t₂ {
+      assume σ x t,
+      assume t_closed,
+      assume h1,
+      rw[vc.subst_env.post],
+      unfold vc.substt,
+      rw[vc.subst_env.post],
+      congr,
+      from term.substt_env.order t_closed h1,
+      from term.substt_env.order t_closed h1
+    },
+    case vc.univ z P' P'_ih {
+      assume σ x t,
+      assume t_closed,
+      assume h1,
+      rw[vc.subst_env.univ],
+      unfold vc.substt,
+      by_cases (x = z) with h2,
+
+      simp[h2],
+      rw[vc.subst_env.univ],
+
+      simp[h2],
+      rw[vc.subst_env.univ],
+      congr,
+
+      have h2: (x ∉ σ.without z),
+      from env.not_in_without h1,
+      have h3: (vc.subst_env (σ.without z) (vc.substt x t P') = vc.substt x t (vc.subst_env (σ.without z) P')),
+      from P'_ih t_closed h2,
+      rw[h3]
+    }
+  end
+
+lemma vc.substte_env.order {P: vc} {x: var} {t: term}:
+    ∀ {σ₁ σ₂: env},
+      (∀z, z ∈ σ₁ → (σ₁ z = σ₂ z)) → (x ∉ σ₁) →
+      (vc.subst_env σ₁ (vc.substte x t P σ₂) = vc.substte x t (vc.subst_env σ₁ P) σ₂) :=
+  begin
+    induction P,
+    case vc.term t' {
+      assume σ₁ σ₂,
+      assume env_equiv,
+      assume x_not_in_σ₁,
+      change (vc.subst_env σ₁ (vc.substte x t (vc.term t') σ₂) = vc.substte x t (vc.subst_env σ₁ t') σ₂),
+      rw[vc.subst_env.term],
+      unfold vc.substte,
+      rw[vc.subst_env.term],
+      congr,
+      from term.substte_env.order env_equiv x_not_in_σ₁
+    },
+    case vc.not P₁ ih {
+      assume σ₁ σ₂,
+      assume env_equiv,
+      assume x_not_in_σ₁,
+      rw[vc.subst_env.not],
+      unfold vc.substte,
+      rw[vc.subst_env.not],
+      congr,
+      from ih env_equiv x_not_in_σ₁
+    },
+    case vc.and P₁ P₂ P₁_ih P₂_ih {
+      assume σ₁ σ₂,
+      assume env_equiv,
+      assume x_not_in_σ₁,
+      change (vc.subst_env σ₁ (vc.substte x t (vc.and P₁ P₂) σ₂) = vc.substte x t (vc.subst_env σ₁ (P₁ ⋀ P₂)) σ₂),
+      rw[vc.subst_env.and],
+      unfold vc.substte,
+      rw[vc.subst_env.and],
+      congr,
+      from P₁_ih env_equiv x_not_in_σ₁,
+      from P₂_ih env_equiv x_not_in_σ₁
+    },
+    case vc.or P₁ P₂ P₁_ih P₂_ih {
+      assume σ₁ σ₂,
+      assume env_equiv,
+      assume x_not_in_σ₁,
+      change (vc.subst_env σ₁ (vc.substte x t (vc.or P₁ P₂) σ₂) = vc.substte x t (vc.subst_env σ₁ (P₁ ⋁ P₂)) σ₂),
+      rw[vc.subst_env.or],
+      unfold vc.substte,
+      rw[vc.subst_env.or],
+      congr,
+      from P₁_ih env_equiv x_not_in_σ₁,
+      from P₂_ih env_equiv x_not_in_σ₁
+    },
+    case vc.pre t₁ t₂ {
+      assume σ₁ σ₂,
+      assume env_equiv,
+      assume x_not_in_σ₁,
+      rw[vc.subst_env.pre],
+      unfold vc.substte,
+      rw[vc.subst_env.pre],
+      congr,
+      from term.substte_env.order env_equiv x_not_in_σ₁,
+      from term.substte_env.order env_equiv x_not_in_σ₁
+    },
+    case vc.pre₁ op t {
+      assume σ₁ σ₂,
+      assume env_equiv,
+      assume x_not_in_σ₁,
+      rw[vc.subst_env.pre₁],
+      unfold vc.substte,
+      rw[vc.subst_env.pre₁],
+      congr,
+      from term.substte_env.order env_equiv x_not_in_σ₁
+    },
+    case vc.pre₂ op t₁ t₂ {
+      assume σ₁ σ₂,
+      assume env_equiv,
+      assume x_not_in_σ₁,
+      rw[vc.subst_env.pre₂],
+      unfold vc.substte,
+      rw[vc.subst_env.pre₂],
+      congr,
+      from term.substte_env.order env_equiv x_not_in_σ₁,
+      from term.substte_env.order env_equiv x_not_in_σ₁
+    },
+    case vc.post t₁ t₂ {
+      assume σ₁ σ₂,
+      assume env_equiv,
+      assume x_not_in_σ₁,
+      rw[vc.subst_env.post],
+      unfold vc.substte,
+      rw[vc.subst_env.post],
+      congr,
+      from term.substte_env.order env_equiv x_not_in_σ₁,
+      from term.substte_env.order env_equiv x_not_in_σ₁
+    },
+    case vc.univ y P' P'_ih {
+      assume σ₁ σ₂,
+      assume env_equiv,
+      assume x_not_in_σ₁,
+      rw[vc.subst_env.univ],
+      unfold vc.substte,
+      by_cases (x = y) with h2,
+
+      simp[h2],
+      rw[vc.subst_env.univ],
+
+      simp[h2],
+      rw[vc.subst_env.univ],
+      congr,
+
+
+      have h3: (∀ (z : var), z ∈ σ₁.without y → ((σ₁.without y) z = (σ₂.without y) z)), by begin
+        assume z: var,
+        assume h4: z ∈ σ₁.without y,
+        have h5, from env.contains_without.inv h4,
+        have h6: (σ₁ z = σ₂ z), from env_equiv z h5.right,
+        have h7, from env.contains_apply_equiv.right.mpr h5.right,
+        rw[h6] at h7,
+        have h8, from env.contains_apply_equiv.right.mp h7,
+        have h9, from env.contains_without.rinv ⟨h8, h5.left⟩,
+        have h10, from env.without_equiv_with z h4,
+        have h11, from env.without_equiv_with z h9,
+        from eq.trans h10 (eq.trans h6 h11.symm)
+      end,
+      have h4: (x ∉ σ₁.without y), from env.not_in_without x_not_in_σ₁,
+      from P'_ih h3 h4
+    }
+  end
+
+lemma vc.subst_env_inner {P: vc} {σ: env} {x: var} {v: value}:
+      (σ x = some v) → (vc.subst_env σ (vc.subst x v P) = vc.subst_env σ P) :=
+  begin
+    assume x_is_v,
+
+    induction σ with σ₁ y v' ih,
+
+    show (vc.subst_env env.empty (vc.subst x v P) = vc.subst_env env.empty P), by cases x_is_v,
+
+    show (vc.subst_env (σ₁[y↦v']) (vc.subst x v P) = vc.subst_env (σ₁[y↦v']) P), by begin
+      unfold vc.subst_env,
+      have h2: (env.apply (σ₁[y↦v']) x = some v), from x_is_v,
+      unfold env.apply at h2,
+      by_cases (y = x ∧ (option.is_none (env.apply σ₁ x))) with h3,
+      simp[h3] at h2,
+      have h4: (v' = v), from option.some.inj h2,
+      simp[h3],
+      have h5: (σ₁ x = none), from option.is_none.inv.mpr h3.right,
+      have h6: x ∉ σ₁, from env.contains_apply_equiv.left.mp h5,
+      rw[h4],
+      have h7: x ∉ FV (vc.subst x v P), from vc.not_free_of_subst,
+      have h8: x ∉ FV (vc.subst_env σ₁ (vc.subst x v P)),
+      from mt free_in_vc.subst_env h7,
+      have h9: (vc.subst x v (vc.subst_env σ₁ (vc.subst x v P)) = (vc.subst_env σ₁ (vc.subst x v P))),
+      from unchanged_of_subst_nonfree_vc h8,
+      rw[h9],
+      from vc.subst_env.order (or.inl h6),
+
+      simp[h3] at h2,
+      have h4, from ih h2,
+      congr,
+      from h4
+    end
+  end
+
+lemma vc.subst_env_with_equivalent_env {P: vc} {σ₁ σ₂: env}:
+  (∀z, z ∈ σ₁ → (σ₁ z = σ₂ z)) → (vc.subst_env σ₂ (vc.subst_env σ₁ P) = vc.subst_env σ₂ P) :=
+  begin
+    assume env_equiv,
+    induction σ₁ with σ₁' x v ih,
+    
+    show (vc.subst_env σ₂ (vc.subst_env env.empty P) = vc.subst_env σ₂ P), from (
+      have vc.subst_env env.empty P = P, by unfold vc.subst_env,
+      show vc.subst_env σ₂ (vc.subst_env env.empty P) = vc.subst_env σ₂ P, from this.symm ▸ rfl
+    ),
+
+    show (vc.subst_env σ₂ (vc.subst_env (σ₁'[x↦v]) P) = vc.subst_env σ₂ P), by begin
+      unfold vc.subst_env,
+
+      have h0: (∀ (z : var), z ∈ σ₁' → (σ₁' z = σ₂ z)), from (
+        assume z: var,
+        assume h1: z ∈ σ₁',
+        have ∃v, σ₁' z = some v, from env.contains_apply_equiv.right.mpr h1,
+        let ⟨v', h2⟩ := this in
+        have option.is_some (σ₁' z), from option.is_some_iff_exists.mpr this,
+        have ¬ option.is_none (σ₁' z), from option.some_iff_not_none.mp this,
+        have ¬ (x = z ∧ option.is_none (env.apply σ₁' z)), from not_and_distrib.mpr (or.inr this),
+        have h3: env.apply (σ₁'[x↦v]) z = σ₁' z, by { unfold env.apply, simp[this], refl },
+        have z ∈ (σ₁'[x↦v]), from env.contains.rest h1,
+        show σ₁' z = σ₂ z, from h3 ▸ (env_equiv z this)
+      ),
+      by_cases (x ∈ σ₁') with h1,
+
+      have h2: x ∉ FV (vc.subst_env σ₁' P), from vc.not_free_of_subst_env h1,
+      have h3: (vc.subst x v (vc.subst_env σ₁' P) = (vc.subst_env σ₁' P)),
+      from unchanged_of_subst_nonfree_vc h2,
+      rw[h3],
+      from ih h0,
+
+      have h2: x ∈ (σ₁'[x↦v]), from env.contains.same,
+      have h3: ((σ₁'[x↦v]) x = σ₂ x), from env_equiv x h2,
+      have h4: (env.apply (σ₁'[x↦v]) x = v), from env.apply_of_contains h1,
+      have h5: (σ₂ x = some v), from eq.trans h3.symm h4,
+      have h6: (vc.subst_env σ₂ (vc.subst x v (vc.subst_env σ₁' P)) = vc.subst_env σ₂ (vc.subst_env σ₁' P)),
+      from vc.subst_env_inner h5,
+      rw[h6],
+      from ih h0
+    end
+  end
+
+lemma vc.subst_env_equivalent_env {P: vc} {σ₁ σ₂: env}:
+  (∀z, z ∈ σ₁ → (σ₁ z = σ₂ z)) → closed_subst σ₁ P → (vc.subst_env σ₁ P = vc.subst_env σ₂ P) :=
+  assume h1: (∀z, z ∈ σ₁ → (σ₁ z = σ₂ z)),
+  assume P_closed: closed_subst σ₁ P,
+  have closed (vc.subst_env σ₁ P), from vc.closed_of_closed_subst P_closed,
+  have h2: vc.subst_env σ₂ (vc.subst_env σ₁ P) = (vc.subst_env σ₁ P),
+  from unchanged_of_subst_env_nonfree_vc this σ₂,
+  have vc.subst_env σ₂ (vc.subst_env σ₁ P) = vc.subst_env σ₂ P,
+  from vc.subst_env_with_equivalent_env h1,
+  show vc.subst_env σ₁ P = vc.subst_env σ₂ P, from h2 ▸ this
+
+lemma env.remove_unimportant_equivalence {σ₁ σ₂: env} {x: var}:
+  (∀y, y ∈ σ₁ → (σ₁ y = σ₂ y)) → x ∉ σ₁ → (∀y, y ∈ σ₁ → (σ₁ y = σ₂.without x y)) :=
+  assume h1: (∀y, y ∈ σ₁ → (σ₁ y = σ₂ y)),
+  assume h2: x ∉ σ₁,
+  assume y: var,
+  assume h3: y ∈ σ₁,
+  have ∃v, σ₁ y = some v, from env.contains_apply_equiv.right.mpr h3,
+  let ⟨v, h4⟩ := this in
+  have σ₁ y = σ₂ y, from h1 y h3,
+  have h5: σ₂ y = v, from eq.trans this.symm h4,
+  have h6: x ≠ y, from (
+    assume : x = y,
+    have x ∈ σ₁, from this.symm ▸ h3,
+    show «false», from h2 this
+  ),
+  have y ∈ σ₁.dom, from h3,
+  have y ∈ σ₂.dom, from set.mem_of_subset_of_mem (env.dom_subset_of_equivalent_env h1) this,
+  have y ∈ σ₂, from this,
+  have h7: y ∈ σ₂.without x, from env.contains_without.rinv ⟨this, h6.symm⟩,
+  -- have ∃v', σ₂.without x y = some v', from env.contains_apply_equiv.right.mpr this,
+  have y ∉ σ₂.without x ∨ (σ₂.without x y = v), from env.without_equiv (or.inr h5),
+  or.elim this (
+    assume : y ∉ σ₂.without x,
+    show σ₁ y = σ₂.without x y, from absurd h7 this
+  ) (
+    assume : σ₂.without x y = v,
+    show σ₁ y = σ₂.without x y, from eq.trans h4 this.symm
+  )
+
+lemma vc.subst_env_without_nonfree {σ: env} {P: vc} {x: var}:
+  x ∉ FV P → (vc.subst_env σ P = vc.subst_env (σ.without x) P) :=
+  begin
+    assume h1: x ∉ FV P,
+
+    induction σ with σ' y v ih,
+
+    show (vc.subst_env env.empty P = vc.subst_env (env.without env.empty x) P), by begin
+      unfold env.without
+    end,
+
+    show (vc.subst_env (σ'[y↦v]) P = vc.subst_env (env.without (σ'[y↦v]) x) P), by begin
+      unfold env.without,
+      by_cases (y = x) with h2,
+
+      simp[h2],
+      unfold vc.subst_env,
+      have h3: x ∉ FV (vc.subst_env σ' P), by begin
+        assume : x ∈ FV (vc.subst_env σ' P),
+        have : x ∈ FV P, from free_in_vc.subst_env this,
+        show «false», from h1 this
+      end,
+      have h4: (vc.subst x v (vc.subst_env σ' P) = (vc.subst_env σ' P)),
+      from unchanged_of_subst_nonfree_vc h3,
+      from eq.trans h4 ih,
+
+      simp[h2],
+      unfold vc.subst_env,
+      rw[ih]
+    end
+  end
+
+lemma vc.subst_env.reorder {σ: env} {x: var} {v: value} {P: vc}:
+  (vc.subst_env σ (vc.subst x v P) = vc.subst x v (vc.subst_env (σ.without x) P)) :=
+  have x ∉ FV (vc.subst x v P), from vc.not_free_of_subst,
+  have h1: vc.subst_env σ (vc.subst x v P) = vc.subst_env (σ.without x) (vc.subst x v P),
+  from vc.subst_env_without_nonfree this,
+  have x ∉ σ.without x, from env.not_contains_without,
+  have h2: (vc.subst_env (σ.without x) (vc.subst x v P) = vc.subst x v (vc.subst_env (σ.without x) P)),
+  from vc.subst_env.order (or.inl this),
+  show vc.subst_env σ (vc.subst x v P) = vc.subst x v (vc.subst_env (σ.without x) P),
+  from eq.trans h1 h2
+
+lemma vc.substt_env.reorder {σ: env} {x: var} {t: term} {P: vc}:
+  closed t → (vc.subst_env σ (vc.substt x t P) = vc.substt x t (vc.subst_env (σ.without x) P)) :=
+  assume t_closed: closed t,
+  have x ∉ FV (vc.substt x t P), from vc.not_free_of_substt t_closed,
+  have h1: vc.subst_env σ (vc.substt x t P) = vc.subst_env (σ.without x) (vc.substt x t P),
+  from vc.subst_env_without_nonfree this,
+  have x ∉ σ.without x, from env.not_contains_without,
+  have h2: (vc.subst_env (σ.without x) (vc.substt x t P) = vc.substt x t (vc.subst_env (σ.without x) P)),
+  from vc.substt_env.order t_closed this,
+  show vc.subst_env σ (vc.substt x t P) = vc.substt x t (vc.subst_env (σ.without x) P),
+  from eq.trans h1 h2
+
+lemma vc.substte_env.reorder {σ: env} {x: var} {t: term} {P: vc}:
+  closed_subst σ t → (vc.subst_env σ (vc.substte x t P σ) = vc.substte x t (vc.subst_env (σ.without x) P) σ) :=
+  assume t_closed: closed_subst σ t,
+  have x ∉ FV (vc.substte x t P σ), from vc.not_free_of_substte t_closed,
+  have h1: vc.subst_env σ (vc.substte x t P σ) = vc.subst_env (σ.without x) (vc.substte x t P σ),
+  from vc.subst_env_without_nonfree this,
+  have h2: (∀z, z ∈ σ.without x → (σ.without x z = σ z)), from env.without_equiv_with,
+  have x ∉ σ.without x, from env.not_contains_without,
+  have h3: (vc.subst_env (σ.without x) (vc.substte x t P σ) = vc.substte x t (vc.subst_env (σ.without x) P) σ),
+  from vc.substte_env.order h2 this,
+  show vc.subst_env σ (vc.substte x t P σ) = vc.substte x t (vc.subst_env (σ.without x) P) σ,
+  from eq.trans h1 h3
+
+lemma term.substt_env.redundant {σ: env} {x: var} {t t': term}:
+  (term.subst_env σ (term.substt x (term.subst_env σ t) t') = term.subst_env σ (term.substt x t t')) :=
+  begin
+    induction t' with v y unop t₁ t₁_ih binop t₂ t₃ t₂_ih t₃_ih t₄ t₅ t₄_ih t₅_ih,
+
+    show (term.subst_env σ (term.substt x (term.subst_env σ t) (term.value v)) =
+          term.subst_env σ (term.substt x t (term.value v))), by begin
+      unfold term.substt
+    end,
+
+    show (term.subst_env σ (term.substt x (term.subst_env σ t) (term.var y)) =
+          term.subst_env σ (term.substt x t (term.var y))), by begin
+      unfold term.substt,
+      by_cases (x = y) with h1,
+      simp[h1],
+      from term.subst_env_twice,
+      simp[h1]
+    end,
+
+    show (term.subst_env σ (term.substt x (term.subst_env σ t) (term.unop unop t₁)) =
+          term.subst_env σ (term.substt x t (term.unop unop t₁))), by begin
+      unfold term.substt,
+      rw[term.subst_env.unop],
+      rw[term.subst_env.unop],
+      congr,
+      from t₁_ih
+    end,
+
+    show (term.subst_env σ (term.substt x (term.subst_env σ t) (term.binop binop t₂ t₃)) =
+          term.subst_env σ (term.substt x t (term.binop binop t₂ t₃))), by begin
+      unfold term.substt,
+      rw[term.subst_env.binop],
+      rw[term.subst_env.binop],
+      congr,
+      from t₂_ih,
+      from t₃_ih
+    end,
+
+    show (term.subst_env σ (term.substt x (term.subst_env σ t) (term.app t₄ t₅)) =
+          term.subst_env σ (term.substt x t (term.app t₄ t₅))), by begin
+      unfold term.substt,
+      rw[term.subst_env.app],
+      rw[term.subst_env.app],
+      congr,
+      from t₄_ih,
+      from t₅_ih
+    end
+  end
+
+-- lemma vc.substt_env.redundant {x: var} {t: term} {P: vc}:
+--   ∀σ, (vc.subst_env σ (vc.substt x (term.subst_env σ t) P) = vc.subst_env σ (vc.substt x t P)) :=
+--   begin
+--     induction P,
+--     case vc.term t' {
+--       assume σ,
+--       unfold vc.substt,
+--       rw[vc.subst_env.term],
+--       rw[vc.subst_env.term],
+--       apply vc.term.inj.inv,
+--       from term.substt_env.redundant
+--     },
+--     case vc.not P₁ ih {
+--       assume σ,
+--       unfold vc.substt,
+--       rw[vc.subst_env.not],
+--       rw[vc.subst_env.not],
+--       apply vc.not.inj.inv,
+--       from ih σ
+--     },
+--     case vc.and P₁ P₂ P₁_ih P₂_ih {
+--       assume σ,
+--       unfold vc.substt,
+--       rw[vc.subst_env.and],
+--       rw[vc.subst_env.and],
+--       apply vc.and.inj.inv,
+--       from P₁_ih σ,
+--       from P₂_ih σ
+--     },
+--     case vc.or P₁ P₂ P₁_ih P₂_ih {
+--       assume σ,
+--       unfold vc.substt,
+--       rw[vc.subst_env.or],
+--       rw[vc.subst_env.or],
+--       apply vc.or.inj.inv,
+--       from P₁_ih σ,
+--       from P₂_ih σ
+--     },
+--     case vc.pre t₁ t₂ {
+--       assume σ,
+--       unfold vc.substt,
+--       rw[vc.subst_env.pre],
+--       rw[vc.subst_env.pre],
+--       apply vc.pre.inj.inv,
+--       from term.substt_env.redundant,
+--       from term.substt_env.redundant
+--     },
+--     case vc.pre₁ op t₁ {
+--       assume σ,
+--       unfold vc.substt,
+--       rw[vc.subst_env.pre₁],
+--       rw[vc.subst_env.pre₁],
+--       apply vc.pre₁.inj.inv,
+--       from term.substt_env.redundant
+--     },
+--     case vc.pre₂ op t₁ t₂ {
+--       assume σ,
+--       unfold vc.substt,
+--       rw[vc.subst_env.pre₂],
+--       rw[vc.subst_env.pre₂],
+--       apply vc.pre₂.inj.inv,
+--       from term.substt_env.redundant,
+--       from term.substt_env.redundant
+--     },
+--     case vc.post t₁ t₂ {
+--       assume σ,
+--       unfold vc.substt,
+--       rw[vc.subst_env.post],
+--       rw[vc.subst_env.post],
+--       apply vc.post.inj.inv,
+--       from term.substt_env.redundant,
+--       from term.substt_env.redundant
+--     },
+--     case vc.univ y P₁ P₁_ih {
+--       assume σ,
+--       unfold vc.substt,
+--       rw[vc.subst_env.univ],
+--       rw[vc.subst_env.univ],
+--       apply vc.univ.inj.inv,
+--       by_cases (x = y) with h1,
+
+--       simp[h1],
+--       simp[h1],
+--       from P₁_ih (σ.without y)
+--     }
+--   end
